\documentclass[12pt]{article}
\pagenumbering{gobble}
\linespread{1.15}

\usepackage{amsfonts}
\usepackage{amsmath}
\usepackage{amssymb}
\usepackage{array}
\usepackage{fancyhdr}
\usepackage{textcomp}
\usepackage[margin=1in,headheight=1in]{geometry}

\newcommand{\contradiction}{
    \ensuremath{{\Rightarrow\mspace{-2mu}\Leftarrow}}
}

\newcommand{\angleb}[1]{\left\langle#1\right\rangle}
\newcommand{\vertb}[1]{\left\vert#1\right\vert}
\newcommand{\bracks}[1]{\left[#1\right]}

\newcommand{\derv}[2]{\dfrac{d#1}{d#2}}
\newcommand{\pderv}[2]{\dfrac{\partial#1}{\partial#2}}

\begin{document}
\pagestyle{fancy}
\fancyhead{}
\fancyhead[L]{Alexander Agruso}
\fancyhead[R]{MATH 3323 Homework 6}

\normalsize
\begin{itemize}
    \item [3.)] Check equation for exactness:
    \[\pderv{M}{y}=\pderv{}{y}\bracks{3x^2-2xy+2}=-2x=\pderv{N}{x}=\pderv{}{x}\bracks{6y^2-x^2+3}=-2x\]
    Integrate $M$ and $N$:
    \[\int 3x^2-2xy+2\ dx=x^3-x^2y+2x+h(y)\]
    \[\int 6y^2-x^2+3\ dy=2y^3-x^2y+3y+g(x)\]
    \[\therefore\ g(x)=x^3+2x,h(y)=2y^3+3y\]
    \[\therefore\ f(x,y)=x^3-x^2y+2x+2y^3+3y=C\]
    Which is the implicit solution.

    \item [9.)] Check equation for exactness:
    \[\pderv{M}{y}=\pderv{}{y}\bracks{2x-y}=-1=\pderv{N}{x}=\pderv{}{x}\bracks{2y-x}=-1\]
    Integrate $M$ and $N$:
    \[\int 2x-y\ dx=x^2-xy+h(y)\]
    \[\int 2y-x\ dy=y^2-xy+g(x)\]
    \[\therefore\ g(x)=x^2,h(y)=y^2\]
    \[\therefore\ f(x,y)=x^2-xy+y^2=C\]
    Solve for $C$ given $y(1)=3$:
    \[1^2-3(1)+1^2=1-3+1=-1=C\]
    \[\therefore\ f(x,y)=x^2-xy+y^2=C\implies y^2-xy+x^2-C=0\]
    \[\implies y=\frac{x\pm\sqrt{x^2-4(x^2-C)}}{2}=\frac{x\pm\sqrt{-3x^2+4}}{2}\]
    Which is the particular solution.

    \pagebreak
    \item [11.)] Take mixed derivatives of $M$ and $N$:
    \[\pderv{M}{y}=\pderv{}{y}\bracks{xy^2+bx^2y}=2xy+bx^2,\pderv{N}{x}=\pderv{}{x}\bracks{x^3+x^2y}=3x^2+2xy\]
    Thus $b=3$, and the equation is exact. Integration $M$ and $N$:
    \[\int xy^2+3x^2y\ dx=\frac{x^2y^2}{2}+x^3y+h(y)\]
    \[\int x^3+x^2y\ dy=x^3y+\frac{x^2y^2}{2}+g(x)\]
    \[\therefore\ g(x)=h(y)=0\]
    \[\therefore\ f(x,y)=x^3y+\frac{x^2y^2}{2}=C\]
    Which is the implicit solution.

    \item [15.)] Check equation for exactness:
    \[\pderv{M}{y}=\pderv{}{y}\bracks{x^2y^3}=3x^2y^2\neq\pderv{N}{x}=\pderv{}{x}\bracks{x+xy^2}=1+y^2\]
    Since the equation is not exact, multiply by given integrating factor $\mu(x,y)=\dfrac{1}{xy^3}$:
    \[\pderv{\mu M}{y}=\pderv{}{y}\bracks{\frac{x^2y^3}{xy^3}}=\pderv{}{y}\bracks{x}=0=\pderv{\mu N}{x}=\pderv{}{x}\bracks{\frac{x+xy^2}{xy^3}}=\pderv{}{x}\bracks{\frac{1}{y^3}+\frac{1}{y}}=0\]
    Thus the equation is exact. Integrate $\mu M$ and $\mu N$:
    \[\int x\ dx=\frac{x^2}{2}+h(y)\]
    \[\int\frac{1}{y^3}+\frac{1}{y}\ dy=\ln\vert y\vert-\frac{1}{2y^2}+g(x)\]
    \[\therefore\ g(x)=\frac{x^2}{2},h(y)=\ln\vert y\vert-\frac{1}{2y^2}\]
    \[\therefore\ f(x,y)=\frac{x^2}{2}+\ln\vert y\vert-\frac{1}{2y^2}=C\]
    Which is the implicit solution.

    \pagebreak
    \item [21.)] Check equation for exactness:
    \[\pderv{M}{y}=\pderv{}{y}\bracks{y}=1\neq\pderv{N}{x}=\pderv{}{x}\bracks{2xy-e^{-2y}}=2y\]
    Thus the equation is not exact. Find integrating factor $\mu$:
    \[\frac{M_y-N_x}{N}=\frac{1-2y}{2xy-e^{-2y}}\text{ is not a function of }x\]
    \[\frac{N_x-M_y}{M}=\frac{2y-1}{y}=2-\frac{1}{y}\]
    \[\therefore\ \mu(y)=e^{\int2-\frac{1}{y}dy}=e^{2y-\ln\vert y\vert}=\frac{e^{2y}}{y}\]
    Multiply the equation by $\mu$ and solve:
    \[\mu M=\frac{ye^{2y}}{y}=e^{2y},\mu N=\frac{e^{2y}(2xy-e^{-2y})}{y}=2xe^{2y}-\frac{1}{y}\]
    \[\int e^{2y}\ dx=xe^{2y}+h(y)\]
    \[\int2xe^{2y}-\frac{1}{y}\ dy=xe^{2y}-\ln\vert y\vert+g(x)\]
    \[\therefore\ g(x)=0,h(y)=-\ln\vert y\vert\]
    \[\therefore\ f(x,y)=xe^{2y}-\ln\vert y\vert=C\]
    Which is the implicit solution.

    \item [1.)] Check equation for exactness:
    \[\pderv{M}{y}=\pderv{}{y}\bracks{2xy^2+2y}=4xy+2=\pderv{N}{x}=\pderv{}{x}\bracks{2x^2y+2x}=4xy+2\]
    Integration $M$ and $N$:
    \[\int2xy^2+2y\ dx=x^2y^2+2xy+h(y)\]
    \[\int2x^2y+2x\ dy=x^2y^2+2xy+g(x)\]
    \[\therefore\ g(x)=h(y)=0\]
    \[\therefore\ f(x,y)=x^2y^2+2xy=C\implies y=\frac{-2x\pm\sqrt{4x^2-4(-Cx^2)}}{2x^2}\]
    \[=-\frac{1}{x}\pm\frac{\sqrt{x^2(1+C)}}{x^2}=\pm\frac{\sqrt{1+C}}{x}-\frac{1}{x}\]
    Which is the explicit solution.

    \pagebreak
    \item [2.)] Check equation for exactness:
    \[\pderv{M}{y}=\pderv{}{y}\bracks{e^x\sin y-2y\sin x}=e^x\cos y-2\sin x\]
    \[=\pderv{N}{x}=\pderv{}{x}\bracks{e^x\cos y+2\cos x}=e^x\cos y-2\sin x\]
    Integrate $M$ and $N$:
    \[\int e^x\sin y-2y\sin x\ dx=e^x\sin y+2y\cos x+h(y)\]
    \[\int e^x\cos y+2\cos x\ dy=e^x\sin y+2y\cos x+g(x)\]
    \[\therefore\ g(x)=h(y)=0\]
    \[\therefore\ f(x,y)=e^x\sin y+2y\cos x=C\]
    Which is the implicit solution.

\end{itemize}

\end{document}
