\documentclass[12pt]{article}
\pagenumbering{gobble}
\linespread{1}

\usepackage{amsfonts}
\usepackage{amsmath}
\usepackage{amssymb}
\usepackage{array}
\usepackage{fancyhdr}
\usepackage{mathtools}
\usepackage{textcomp}
\usepackage[margin=1in,headheight=10mm]{geometry}

\newcommand{\contradiction}{%
    \ensuremath{{\Rightarrow\mspace{-2mu}\Leftarrow}}%
}

\newcommand{\angleb}[1]{\left\langle#1\right\rangle}
\newcommand{\vertb}[1]{\left\vert#1\right\vert}
\newcommand{\bracks}[1]{\left[#1\right]}
\newcommand{\parns}[1]{\left(#1\right)}
\newcommand{\dvert}[1]{\left\Vert#1\right\Vert}

\begin{document}
\pagestyle{fancy}
\fancyhead{}
\fancyhead[L]{Alexander Agruso}
\fancyhead[R]{MATH 2393 Homework 6}

\normalsize
\section*{Exercises 15.1}
\begin{itemize}
    \item [15.)] \[\int^4_1\int^2_0\left(6x^2y-2x\right)\,dy\,dx=\int_{1}^{4}\bracks{3x^2y^2-2xy}^2_0\,dx=\int_{1}^{4}12x^2-4x\,dx\]
    \[=\bracks{4x^3-2x^2}^4_1=256-32-4+2=222\]

    \item [19.)] \[\int^3_{-3}\int^{\pi/2}_0(y+y^2\cos x)\,dx\,dy=\int^3_{-3}\bracks{xy+y^2\sin x}^{\pi/2}_0=\int^3_{-3}\frac{\pi}{2}y+y^2\,dy\]
    \[=\bracks{\frac{\pi}{4}y^2+\frac{y^3}{3}}^3_{-3}=\frac{9\pi}{4}+9-\frac{9\pi}{4}+9=18\]

    \item [29.)] \[\iint\limits_R\frac{xy^2}{x^2+1}\,dA=\int^3_{-3}\int^1_0\frac{xy^2}{x^2+1}\,dx\,dy=\frac{1}{2}\int^3_{-3}\int^1_0\frac{y^2}{u}\,du\,dy=\frac{1}{2}\int^3_{-3}\bracks{y^2\ln\vert u\vert}^1_0\]
    \[=\frac{1}{2}\int^3_{-3}\bracks{y^2\ln\vert x^2+1\vert}^1_0=\frac{1}{2}\int^3_{-3}\bracks{y^2\ln2}\,dy=\frac{\ln2}{2}\bracks{\frac{y^3}{3}}^3_{-3}=\frac{18\ln2}{2}=9\ln2\]

    \item [33.)] \[\iint\limits_Rye^{-xy}\,dA=\int^3_0\int^2_0ye^{-xy}\,dx\,dy=\int^3_0\bracks{-e^{-xy}dy}^2_0=\int^3_{0}-e^{-2y}+e^0\,dy\]
    \[\int^3_{0}1-e^{-2y}\,dy=\bracks{y+\frac{e^{-2y}}{2}}^3_0=3+\frac{e^{-6}}{2}-\frac{1}{2}=\frac{e^{-6}+5}{2}\]

    \item [41.)] Find the limits:
    \[-1\leq x\leq1,\ 0\leq y\leq1\]
    Evaluate the integral:
    \[\int^1_{-1}\int^1_01+x^2ye^y\,dx\,dy=\int^1_{-1}\bracks{x+\frac{x^3ye^y}{3}}^1_0\,dy=\int^1_{-1}1+\frac{ye^y}{3}\,dy\]
    \[=\bracks{y+\frac{ye^y}{3}-\frac{e^y}{3}}^1_{-1}=1+\frac{e}{3}-\frac{e}{3}+1+\frac{1}{3e}+\frac{1}{3e}=2+\frac{2}{3e}\]

\end{itemize}

\section*{Exercises 15.2}
\begin{itemize}
    \item [3.)] \[\int^1_0\int^y_0xe^{y^3}\,dx\,dy=\int^1_0\bracks{\frac{x^2e^{y^3}}{2}}^y_0\,dy=\int^1_0\frac{y^2e^{y^3}}{2}\,dy=\frac{1}{6}\bracks{e^u}^1_0=\frac{1}{6}\bracks{e^{y^3}}^1_0=\frac{e-1}{6}\]

    \item [13.)] \[\iint\limits_Dx\,dA=\int^1_0\int^x_0x\,dy\,dx=\int^1_0\bracks{xy}^x_0\,dx=\int^1_0x^2\,dx=\bracks{\frac{x^3}{3}}^1_0=\frac{1}{3}\]
    \[\iint\limits_Dx\,dA=\int^1_0\int^1_yx\,dx\,dy=\int^1_0\bracks{\frac{x^2}{2}}^1_y\,dx=\int^1_0\frac{1}{2}-\frac{y^2}{2}\,dx=\bracks{\frac{y}{2}-\frac{y^3}{6}}^1_0=\frac{1}{2}-\frac{1}{6}=\frac{1}{3}\]

    \item [15.)] \[\iint\limits_Dy\,dA=\int^2_{-1}\int_{y^2}^{y+2}y\,dx\,dy=\int^2_{-1}\bracks{xy}^{y+2}_{y^2}=\int^2_{-1}2y+y^2-y^3\,dy\]
    \[=\bracks{y^2+\frac{y^3}{3}-\frac{y^4}{4}}^2_{-1}=4+\frac{8}{3}-\frac{16}{4}-1+\frac{1}{3}+\frac{1}{4}=3-1+\frac{1}{4}=\frac{9}{4}\]
    Integrating with respect to $x$ first is easier as it prevents us from having to evaluate two double integrals.

    \item [17.)] \[\iint\limits_Dx\cos y\,dA=\int^1_0\int^{x^2}_0x\cos y\,dy\,dx=-\int^1_0\bracks{x\sin y}^{x^2}_0\,dx=-\int^1_0x\sin x^2\,dx\]
    \[=-\frac{1}{2}\int^1_0\sin u\,du=-\frac{1}{2}\bracks{\cos u}^1_0=-\frac{1}{2}(\cos(1)-1)=\frac{1-\cos(1)}{2}\]

    \item [23.)] \[\iint\limits_D3x+2y\,dy\,dx=\int^1_0\int^{\sqrt x}_{x^2}3x+2y\,dy\,dx=\int^1_0\bracks{3xy+y^2}^{\sqrt x}_{x^2}\,dx\]\[=\int^1_03x^{3/2}+x-3x^3-x^4\,dx=\bracks{\frac{6x^{5/2}}{5}+\frac{x^2}{2}-\frac{3x^4}{4}-\frac{x^5}{5}}=\frac{6}{5}+\frac{1}{2}-\frac{3}{4}-\frac{1}{5}=1-\frac{1}{4}=\frac{3}{4}\]

    \pagebreak
    \item [45.)] 

    \item [53.)] \[\int^1_0\int^1_{\sqrt x}\sqrt{y^3+1}\,dy\,dx=\int^1_0\int^{y^2}_0\sqrt{y^3+1}\,dx\,dy=\int^1_0\bracks{x\sqrt{y^3+1}}^{y^2}_0\,dy\]
    \[=\int^1_0y^2\sqrt{y^3+1}\,dy=\frac{1}{3}\int^1_0\sqrt{u}\,du=\frac{1}{3}\bracks{\frac{2\sqrt{u^3}}{3}}^1_0=\frac{1}{3}\bracks{\frac{2\sqrt{\parns{y^3+1}^3}}{3}}^1_0=\]
    \[\frac{1}{3}\bracks{\frac{2\sqrt8-2}{3}}=\frac{2\parns{\sqrt8-1}}{9}\]

    \item [61.)] Find area of region of integration:
    \[A=\frac{1}{2}bh=\frac{1}{2}(1)(3)=\frac{3}{2}\]
    Now evaluate the integral:
    \[I=\int^1_0\int^{3x}_0xy\,dy\,dx=\int^1_0\bracks{\frac{xy^2}{2}}^{3x}_0\,dx=\int^1_0\frac{9x^3}{2}\,dx=\bracks{\frac{9x^3}{8}}^1_0=\frac{9}{8}\]
    Finally, evaluate $I/A$:
    \[I/A=\frac{9}{8}\times\frac{2}{3}=\frac{18}{24}=\frac{3}{4}\]

\end{itemize}

\section*{Exercises 15.3}
\begin{itemize}
    \item [5.)] \[\int^{3\pi/4}_{\pi/4}\int^2_1r\,dr\,d\theta=\int^{3\pi/4}_{\pi/4}\bracks{\frac{r^2}{2}}^2_1\,d\theta=\int^{3\pi/4}_{\pi/4}\frac{3}{2}\,d\theta=\frac{3}{2}\bracks{\theta}^{3\pi/4}_{\pi/4}=\frac{3\pi}{4}\]

    \item [7.)] Given $x=r\cos\theta$ and $y=r\sin\theta$, we can convert $f(x,y)$:
    \[x^2y=r^2\cos^2\theta r\sin\theta=r^3\cos^2\theta\sin\theta\]
    Thus we can evaluate the integral:
    \[\int^\pi_0\int^5_0 r^4\cos^2\theta\sin\theta\,dr\,d\theta=\int^\pi_0\bracks{\frac{r^5}{5}\cos^2\theta\sin\theta}^5_0\,d\theta=\frac{5^5}{5}\int^\pi_0\cos^2\theta\sin\theta\,d\theta\]
    \[=-625\int^\pi_0u^2\,du=-625\bracks{\frac{u^3}{3}}^\pi_0=-\frac{625\cos\pi}{3}=\frac{625}{3}***\]

    \item [19.)] \[I=\int^{2\pi}_0\int^5_0r^2\,dr\,d\theta=\int^{2\pi}_0\bracks{\frac{r^3}{3}}^5_0\,d\theta=\int^{2\pi}_0\frac{125}{3}\,d\theta=\frac{125}{3}\bracks{\theta}^{2\pi}_0=\frac{250\pi}{3}\]

    \item [29.)]

\end{itemize}

\section*{Exercises 15.4}
\begin{itemize}
    \item [17.)] \[I_x=\int^3_1\int^4_1y^4k\,dy\,dx=\int^3_1\bracks{\frac{1}{5}y^5k}^4_1\,dx=\int^3_1\parns{\frac{1023}{5}k}\,dx\]
    \[\frac{1023}{5}\bracks{xk}^3_1=\frac{2(1023)}{5}k=409.2k\]
    \[I_y=\int^3_1\int^4_1x^2ky^2\,dy\,dx=\int^3_1\bracks{\frac{1}{3}x^2ky^3}^4_1\,dx=\int^3_121x^2k\,dx\]
    \[=7\bracks{x^3k}^3_1=7(27k-1k)=7(26k)=182k\]
    \[I_0=\int^3_1\int^4_1(x^2+y^2)ky^2\,dy\,dx=I_x+I_y=591.2k\]

\end{itemize}

\section*{Exercises 15.9}
\begin{itemize}
    \item [1.)] \[J=\begin{vmatrix*}[r]
        2 & 4 \\
        1 & -1
    \end{vmatrix*}=-2-4=-6\]

    \item [3.)] \[J=\begin{vmatrix*}
        \cos t & \sin t \\
        -s\sin t & s\cos t
    \end{vmatrix*}=s\cos^2t+s\sin^2t=s\]

    \item [15.)] First, we can find the bounds of integration for variables $u$ and $v$:
    \[y=2x\implies u+2v=4u+2v\implies u=4u\implies u=0\]
    \[y=\frac{1}{2}x\implies u+2v=u+\frac{1}{2}v\implies 2v=\frac{1}{2}v\implies v=0\]
    \[y=3-x\implies u+2v=3-2u+v\implies 3u=3-3v\implies u=1-v\]
    Now find $J(u,v)$:
    \[J=\begin{vmatrix*}
        2 & 1 \\
        1 & 2
    \end{vmatrix*}=4-1=3\]
    Finally, evaluate the integral:
    \[I=\int^1_0\int^{1-v}_0x-3y\,du\,dv=\int^1_0\int^{1-v}_02u+v-3u-6v\,du\,dv=\int^1_0\bracks{-\frac{u^2}{2}-5uv}^{1-v}_0\]
    \[=\int^1_0-\frac{(1-v)^2}{2}-5(v-1)v\,dv=\frac{1}{2}\int^1_0-v^2+2v-1-10v-10\,dv=\frac{1}{2}\int^1_0-v^2-8v-11\,dv\]
    \[=\frac{1}{2}\bracks{-\frac{v^3}{3}-4v^2-11v}^1_0=\frac{1}{2}\parns{-\frac{1}{3}-4-11}\]

    \item [17.)] awd

\end{itemize}

\end{document}
