\documentclass[12pt]{article}
\pagenumbering{gobble}

\usepackage{amsfonts}
\usepackage{amsmath}
\usepackage{amssymb}
\usepackage{array}
\usepackage{fancyhdr}
\usepackage{mathtools}
\usepackage{textcomp}
\usepackage[margin=1in,headheight=1in]{geometry}

\newcommand{\contradiction}{
    \ensuremath{{\Rightarrow\mspace{-2mu}\Leftarrow}}
}

\newcommand{\angleb}[1]{\left\langle#1\right\rangle}
\newcommand{\vertb}[1]{\left\vert#1\right\vert}
\newcommand{\bracks}[1]{\left[#1\right]}
\newcommand{\parns}[1]{\left(#1\right)}

\newcommand{\derv}[2]{\dfrac{d#1}{d#2}}
\newcommand{\pderv}[2]{\dfrac{\partial#1}{\partial#2}}

\begin{document}
\pagestyle{fancy}
\fancyhead{}
\fancyhead[L]{Alexander Agruso}
\fancyhead[R]{MATH 3323 Homework 12}

\normalsize
\section*{Section 3.2}
\begin{itemize}
    \item [17.)] Find the characteristic equation and the general solution:
    \[y''+y'-2y=0\implies r^2+r-2=(r+2)(r-1)\implies r_1=-2,\ r_2=1\]
    \[\therefore\ y=c_1e^{-2t}+c_2e^t\text{ and }y'=-2c_1e^{-2t}+c_2e^t\]
    Solve for $c_1$ and $c_2$ given $y(t_0)=1,\ y'(t_0)=0$:
    \[1=c_1e^{-2(0)}+c_2e^0=c_1+c_2\]
    \[0=-2c_1e^{-2(0)}+c_2e^0=-2c_1+c_2\]
    \[\therefore\ c_1=\frac{1}{3},\ c_2=\frac{2}{3}\]
    \[\therefore\ y_1=\frac{1}{3}e^{-2t}+\frac{2}{3}e^t\]
    Now solve for $c_1$ and $c_2$ given $y(t_0)=0,\ y'(t_0)=1$:
    \[0=c_1e^{-2(0)}+c_2e^0=c_1+c_2\]
    \[1=-2c_1e^{-2(0)}+c_2e^0=-2c_1+c_2\]
    \[\therefore\ c_1=-\frac{1}{3},\ c_2=\frac{1}{3}\]
    \[\therefore\ y_2=\frac{1}{3}e^t-\frac{1}{3}e^{-2t}\]
    Thus $y_1$ and $y_2$ comprise the fundamental set described by theorem 3.2.5

    \item [18.)] Find the characteristic equation and the general solution:
    \[y''+4y'+3y=0\implies r^2+4r+3=(r+3)(r+1)\implies r_1=-3,r_2=-1\]
    \[y=c_1e^{-3t}+c_2e^{-t}\text{ and }y'=-3c_1e^{-3t}-c_2e^{-t}\]
    Solving for $c_1$ and $c_2$ given $y(t_0)=1,\ y'(t_0)=0$:
    \[1=c_1e^{-3(1)}+c_2e^{-1}=c_1e^{-3}+c_2e^{-1}\]
    \[0=-3c_1e^{-3(1)}-c_2e^{-1}=-3c_1e^{-3}-c_2e^{-1}\]
    \[\therefore\ c_1=-\frac{1}{2e^3},\ c_2=\frac{3}{2e}\]
    \[\therefore\ y_1=\frac{3}{2}e^{-(t+1)}-\frac{1}{2}e^{-3(t+1)}\]
    Now solve for $c_1$ and $c_2$ given $y(t_0)=0,\ y'(t_0)=1$:
    \[0=c_1e^{-3}+c_2e^{-1}\]
    \[1=-3c_1e^{-3}-c_2e^{-1}\]
    \[\therefore\ c_1=-\frac{e^3}{2},\ c_2=\frac{e}{2}\]
    \[\therefore\ y_2=\frac{1}{2}e^{-t+1}-\frac{1}{2}e^{-3t+3}\]
    Thus $y_1$ and $y_2$ comprise the fundamental set described by theorem 3.2.5
\end{itemize}
\section*{Section 3.4}
\begin{itemize}
    \item [18.)] Let $y=v(t)y_1$:
    \[y=v(t)y_1=v(t)t^2,\ y'=v'(t)t^2+2tv(t)\]
    \[y''=v''(t)t^2+2tv'(t)+2v(t)+2tv'(t)=t^2v''(t)+4tv'(t)+2v(t)\]
    \[\therefore\ t^2y''-4ty'+6y=t^2\bracks{t^2v''(t)+4tv'(t)+2v(t)}-4t\bracks{v'(t)t^2+2tv(t)}+6v(t)t^2\]
    \[=t^4v''(t)+4t^3v'(t)-4t^3v'(t)+2t^2v(t)+6t^2v(t)-8t^2v(t)=t^4v''(t)=0\]
    Let $w(t)=v'(t)$:
    \[t^4v''(t)=t^4w'(t)=0\implies w'(t)=0\implies w(t)=v'(t)=c_1\]
    \[\implies v(t)=c_1t+c_2\]
    \[\therefore\ y=(c_1t+c_2)y_1=c_1t^3+c_2t^2\]
    Thus $y_2=t^3$ is another solution to the equation.

    \item [19.)] Let $y=v(t)y_1$:
    \[y=tv(t),\ y'=v(t)+tv'(t),\ y''=v'(t)+v'(t)+tv''(t)=2v'(t)+tv''(t)\]
    \[\therefore\ t^2y''+2ty'-2y=t^2\bracks{2v'(t)+tv''(t)}+2t\bracks{v(t)+tv'(t)}-2tv(t)\]
    \[=2t^2v'(t)+t^3v''(t)+2tv(t)+2t^2v'(t)-2tv(t)=t^3v''(t)+4t^2v'(t)\]
    \[=tv''(t)+4v'(t)=0\]
    Let $w(t)=v'(t)$:
    \[tv''(t)+4v'(t)=tw'(t)+4w(t)=0\implies w'(t)+\frac{4}{t}w(t)=0\]
    \[\mu(t)=e^{\int p(t)dt}=e^{4\ln\vert t\vert}=t^4\]
    \[\therefore w(t)=v'(t)=\frac{1}{\mu(t)}\int \mu(t)g(t)\ dt=\frac{1}{t^4}\int 0t^4=\frac{c_1}{t^4}\]
    \[\therefore\ v(t)=\int\frac{c_1}{t^4}\ dt=-\frac{c_1}{3t^3}+c_2\]
    \[\therefore\ y=v(t)y_1=\parns{c_2-\frac{c_1}{3t^3}}t=c_2t-\frac{c_1t}{3t^3}=c_2t-\frac{c_1}{t^2}\]
    Thus $y_2=t^{-2}$ is another solution to the equation.
    
    \pagebreak
    \item [20.)] Let $y=v(t)y_1$:
    \[y=t^{-1}v(t),\ y'=-t^{-2}v(t)+t^{-1}v'(t),\ y''=2t^{-3}v(t)-t^{-2}v'(t)-t^{-2}v'(t)+t^{-1}v''(t)\]
    \[\therefore\ t^2y''+3ty'+y=t^2\bracks{t^{-1}v''(t)-2t^{-2}v'(t)+2t^{-3}v(t)}+3t\bracks{t^{-1}v'(t)-t^{-2}v(t)}+t^{-1}v(t)\]
    \[=tv''(t)-2v'(t)+2t^{-1}v(t)+3v'(t)-3t^{-1}v(t)+t^{-1}v(t)=tv''(t)+v'(t)=0\]
    Let $w(t)=v'(t)$:
    \[tv''(t)+v'(t)=tw'(t)+w(t)=0\implies w'(t)+\frac{1}{t}w(t)=0\]
    \[\mu(t)=e^{\int p(t)dt}=e^{\ln\vert t\vert}=t\]
    \[\therefore\ w(t)=v'(t)=\frac{1}{t}\int0t\ dt=\frac{c_1}{t}\]
    \[\therefore\ v(t)=\int\frac{c_1}{t}\ dt=c_1\ln\vert t\vert+c_2\]
    \[\therefore\ y=v(t)y_1=\parns{c_1\ln\vert t\vert+c_2}t^{-1}=c_1t^{-1}\ln\vert t\vert+c_2t^{-1}\]
    Thus $y_2=t^{-1}\ln\vert t\vert=t^{-1}\ln t$ is also a solution to the equation.
\end{itemize}
\end{document}
