\documentclass[11pt]{article}
\pagenumbering{gobble}
\linespread{1.25}

\usepackage{amsfonts}
\usepackage{amsmath}
\usepackage{amssymb}
\usepackage{array}
\usepackage{fancyhdr}
\usepackage{mathrsfs}
\usepackage{mathtools}
\usepackage{textcomp}
\usepackage[margin=1in,headheight=1in]{geometry}

\newcommand{\done}{\ensuremath{
    \strut\hfill\blacksquare
}}

\newcommand{\contradiction}{
    \ensuremath{{\Rightarrow\mspace{-2mu}\Leftarrow}}
}

% bracket commands
\newcommand{\angleb}[1]{\left\langle#1\right\rangle} % <>
\newcommand{\vertb}[1]{\left\vert#1\right\vert}      % ||
\newcommand{\bracks}[1]{\left[#1\right]}             % []
\newcommand{\braces}[1]{\left\{#1\right\}}           % {}
\newcommand{\parens}[1]{\left(#1\right)}             % ()

% set aliases
\newcommand{\N}{\mathbb{N}}
\newcommand{\Z}{\mathbb{Z}}
\newcommand{\Q}{\mathbb{Q}}
\newcommand{\R}{\mathbb{R}}

\newcommand{\derv}[2]{\dfrac{d#1}{d#2}}
\newcommand{\e}{\varepsilon}
\newcommand{\di}{\,/\,}

\newcommand{\lm}[1]{\displaystyle\lim_{#1}}

\begin{document}
\pagestyle{fancy}
\fancyhead{}
\fancyhead[L]{Alex Agruso}
\fancyhead[R]{Analysis Homework 7}

\normalsize

\begin{itemize}
    \item [8.2.9] Given $f(x)=x^{-2}$ and a partition $\pi$ of $[a,b]$, we can calculate the following riemann sum with associated points $\xi_k=\sqrt{x_kx_{k-1}}$:
    \[\sum_{k=1}^1f(\xi_k)(x_k-x_{k-1})=\frac{1}{\parens{\sqrt{x_1x_0}}^2}(x_1-x_0)=\frac{x_1-x_0}{x_1x_0}\]
    Now assume that the following equality holds:
    \[\sum_{k=1}^mf(\xi_k)(x_k-x_{k-1})=\frac{x_m-x_0}{x_mx_0}\]
    We can compute the sum to $m+1$ as follows:
    \[\sum_{k=1}^{m+1}f(\xi_k)(x_k-x_{k-1})=\sum_{k+1}^mf(\xi_k)(x_k-x_{k-1})+f(\xi_{m+1})(x_{m+1}-x_m)=\frac{x_m-x_0}{x_mx_0}+\frac{x_{m+1}-x_m}{x_{m+1}x_m}\]
    \[=\frac{x_{m+1}x_m-x_{m+1}x_0+x_{m+1}x_0-x_mx_0}{x_{m+1}x_mx_0}=\frac{x_m(x_{m+1}-x_0)}{x_{m+1}x_mx_0}=\frac{x_{m+1}-x_0}{x_{m+1}x_0}\]
    Thus by induction, we know that
    \[\sum_{k=1}^nf(\xi_k)(x_k-x_{k-1})=\frac{x_n-x_0}{x_nx_0}=\frac{b-a}{ab}\]
    Which is equal to the definite integral $\int_a^bx^{-2}dx$. \done

    \item [8.2.12] By the definition of the definite integral, given a continuous function $f$ defined on $[0,1]$, the following limit can be expressed as a definite integral:
    \[\lm{n\to\infty}\frac{1}{n}\sum_{k=1}^nf\parens{\frac{n}{k}}=\lm{n\to\infty}\frac{1-0}{n}\sum_{k=1}^nf\parens{0+\frac{n}{k}(1-0)}=\int_0^1f(x)dx\]
    \done
\end{itemize}

\end{document}
