\documentclass[12pt]{article}
\pagenumbering{gobble}
\linespread{1.15}

\usepackage{amsfonts}
\usepackage{amsmath}
\usepackage{amssymb}
\usepackage{array}
\usepackage{fancyhdr}
\usepackage{mathtools}
\usepackage{textcomp}
\usepackage[margin=1in,headheight=1in]{geometry}

\newcommand{\contradiction}{
    \ensuremath{{\Rightarrow\mspace{-2mu}\Leftarrow}}
}

\newcommand{\angleb}[1]{\left\langle#1\right\rangle}
\newcommand{\vertb}[1]{\left\vert#1\right\vert}
\newcommand{\bracks}[1]{\left[#1\right]}

\newcommand{\derv}[2]{\dfrac{d#1}{d#2}}
\newcommand{\pderv}[2]{\dfrac{\partial#1}{\partial#2}}

\begin{document}
\pagestyle{fancy}
\fancyhead{}
\fancyhead[L]{Alexander Agruso}
\fancyhead[R]{MATH 3323 Homework 9}

\normalsize
\section*{Section 3.1}
\begin{itemize}
    \item [1.)] Setup and solve the characteristic equation:
    \[y''+2y'-3y=0\to r^2+2r-3=(r-1)(r+3)=0\implies r=1,-3\]
    Since $r_1\neq r_2$, the general solution of the equation is given as
    \[y(t)=c_1e^t+c_2e^{-3t}\]

    \item [2.)] Setup and solve the characteristic equation:
    \[y''+3y'+2y\to r^2+3r+2=(r+1)(r+2)=0\implies r=-1,-2\]
    Since $r_1\neq r_2$, the general solution of the equation is given as
    \[y(t)=c_1e^{-t}+c_2e^{-2t}\]

    \item [9.)] Setup and solve the characteristic equation:
    \[y''+3y'=0\to r^2+3y=r(r+3)\implies r=0,-3\]
    Since $r_1\neq r_2$, the general solution of the equation is given as
    \[y(t)=c_1e^0+c_2e^{-3t}=c_1+c_2e^{-3t}\]
    Solving for $c_1$ and $c_2$ given $y(0)=-2$, $y'(0)=3$ we find the particular solution:
    \[-2=c_1+c_2e^0=c_1+c_2\]
    \[3=-3c_2e^0=-3c_2\]
    \[\implies\bracks{\begin{array}{rr|r}
        1 & 1 & -2\\
        0 & -3 & 3
    \end{array}}\implies\bracks{\begin{array}{rr|r}
        1 & 1 & -2\\
        0 & -1 & 1
    \end{array}}\implies\bracks{\begin{array}{rr|r}
        1 & 0 & -1\\
        0 & -1 & 1
    \end{array}}\]
    \[\implies\bracks{\begin{array}{rr|r}
        1 & 0 & -1\\
        0 & 1 & -1
    \end{array}}\implies c_1=c_2=-1\]
    \[\therefore\ y(t)=-1-e^{-3t}\]
    As $t\to\infty$, $y\to-1$.

    \item [13.)] Determine $r_1$ and $r_2$:
    \[y=c_1e^{2t}+c_2e^{-3t}\implies r_1=2,r_2=-3\]
    \[\therefore\ (r-2)(r+3)=r^2+t-6=0\]
    And derive the equation from its characteristic equation:
    \[y''+y'-6y=0\]

\end{itemize}
\section*{Section 3.3}
\begin{itemize}
    \item [5.)] Setup and solve the characteristic equation:
    \[y''-2y'+2y\to r^2-2r+2=0\]
    \[\frac{2\pm\sqrt{4-4(2)}}{2}=\frac{2\pm\sqrt{-4}}{2}=1\pm i\]
    \[\therefore\ r_1=1+i,r_2=1-i\]
    And find the general solution to the equation:
    \[y(t)=c_1e^{t}\cos t+c_2e^{t}\sin t\]
    \item [12.)] Setup and solve the characteristic equation:
    \[y''+4y=0\to r^2+4=0\]
    \[\frac{\pm\sqrt{-4(4)}}{2}=\frac{\pm{\sqrt{-16}}}{2}=\pm2i\]
    \[\therefore\ r_1=2i,r_2=-2i\]
    And find the general solution to the equation:
    \[y(t)=c_1e^0\cos(2t)+c_2e^0\sin(2t)=c_1\cos(2t)+c_2\sin(2t)\]
    Solving for $c_1$ and $c_2$ given $y(0)=0,y'(0)=1$, we find the particular solution:
    \[0=c_1\cos(2(0))+c_2\sin(2(0))=c_1\]
    \[1=-2c_1\sin(2(0))+2c_2\cos(2(0))=2c_2\implies c_2=\frac{1}{2}\]
    \[\therefore\ y(t)=\frac{1}{2}\sin(2t)\]
    As $t\to\infty$, $y(t)$ will oscillate.
\end{itemize}
\section*{Section 3.4}
\begin{itemize}
    \item [1.)] Setup and solve the characteristic equation:
    \[y''-2y'+y=0\to r^2-2r+1=(r-1)^2=0\]
    \[\therefore\ r_1=r_2=1\]
    Since $r_1=r_2$, the general solution to the equation is given as
    \[y(t)=c_1e^t+c_2te^t\]

    \item [2.)] Setup and solve the characteristic equation:
    \[9y''+6y'+y=0\to 9r^2+6r+1=(3r+1)^2=0\]
    \[\therefore\ r_1=r_2=-\frac{1}{3}\]
    Since $r_1=r_2$, the general solution to the equation is given as
    \[y(t)=c_1e^{-\frac{1}{3}t}+c_2te^{-\frac{1}{3}t}\]

    \item [10.)] Setup and solve the characteristic equation:
    \[y''-6y'+9y=0\to r^2-6r+9=(r-3)^2=0\]
    \[\therefore\ r_1=r_2=3\]
    Since $r_1=r_2$, the general solution to the equation is given as
    \[y(t)=c_1e^{3t}+c_2te^{3t}\]
    Solving for $c_1$ and $c_2$ given $y(0)=0,y'(0)=2$, we find the particular solution:
    \[0=c_1e^0+c_2(0)e^0=c_1\]
    \[2=3c_1e^{0}+c_2(0+e^{0})\implies c_2=2\]
    \[\therefore\ y(t)=(0)e^{3t}+2te^{3t}=2te^{3t}\]
    As $t\to\infty$, $y\to\infty$.
\end{itemize}
\end{document}
