\documentclass[12pt]{article}
\pagenumbering{gobble}

\usepackage{amsfonts}
\usepackage{amsmath}
\usepackage{amssymb}
\usepackage{array}
\usepackage{fancyhdr}
\usepackage{mathtools}
\usepackage{textcomp}
\usepackage[margin=1in,headheight=1in]{geometry}

\newcommand{\contradiction}{
    \ensuremath{{\Rightarrow\mspace{-2mu}\Leftarrow}}
}

\newcommand{\angleb}[1]{\left\langle#1\right\rangle}
\newcommand{\vertb}[1]{\left\vert#1\right\vert}
\newcommand{\bracks}[1]{\left[#1\right]}
\newcommand{\parns}[1]{\left(#1\right)}

\newcommand{\lp}{\mathcal{L}}
\newcommand{\lpi}{\mathcal{L}^{-1}}

\newcommand{\derv}[2]{\dfrac{d#1}{d#2}}
\newcommand{\pderv}[2]{\dfrac{\partial#1}{\partial#2}}

\begin{document}
\pagestyle{fancy}
\fancyhead{}
\fancyhead[L]{Alexander Agruso}
\fancyhead[R]{MATH 3323 Homework 19}

\normalsize
\begin{itemize}
    \item [a.)] \[\lpi\bracks{\frac{s}{(s+3)(s-2)}}=\frac{1}{5}\lpi\bracks{\frac{3}{s+3}+\frac{2}{s-2}}=\frac{3}{5}e^{-3t}+\frac{2}{5}e^{2t}\]

    \item [b.)] \[\lpi\bracks{\frac{1}{s(s+2)}}=\frac{1}{2}\lpi\bracks{\frac{1}{s}-\frac{1}{s+2}}=\frac{1}{2}-\frac{1}{2}e^{-2t}\]

    \item [c.)] \[\lpi\bracks{\frac{s^2}{(s^2-1)(s^2+4)}}=\frac{1}{5}\lpi\bracks{\frac{4}{s^2+4}+\frac{1}{s^2-1}}=\frac{1}{5}\bracks{\frac{4}{s^2+4}+\frac{1}{(s-1)(s+1)}}\]
    \[=\frac{1}{5}\bracks{\frac{4}{s^2+4}+\frac{1}{2}\bracks{\frac{1}{s-1}-\frac{1}{s+1}}}=\frac{1}{5}\cdot\frac{4}{s^2+4}+\frac{1}{10}\cdot\frac{1}{s-1}-\frac{1}{10}\cdot\frac{1}{s+1}\]
    \[=\frac{2}{5}\sin(2t)+\frac{1}{10}e^t-\frac{1}{10}e^{-t}\]

    \item [d.)] \[\lpi\bracks{\frac{1}{s(s^2+4)}}=\int^t_0\lpi\bracks{\frac{1}{s^2+4}}\,dt=\frac{1}{2}\int^t_0\sin(2t)\,dt=-\frac{1}{4}\cos(2t)-\frac{1}{4}\]

    \item [e.)] \[\lpi\bracks{\frac{s}{(s^2+4)(s^2+9)}}=\frac{1}{5}\lpi\bracks{\frac{s}{s^2+4}-\frac{s}{s^2+9}}=\frac{1}{5}\cos(2t)-\frac{1}{5}\cos(3t)\]

    \item [f.)] \[\lpi\bracks{\frac{1}{s^4-16}}=\lpi\bracks{\frac{1}{(s^2-4)(s^2+4)}}=\frac{1}{8}\lpi\bracks{\frac{1}{s^2-4}-\frac{1}{s^2+4}}\]
    \[=\frac{1}{8}\lpi\bracks{\frac{1}{(s-2)(s+2)}-\frac{1}{s^2+4}}=\frac{1}{8}\lpi\bracks{\frac{1}{4}\bracks{\frac{1}{s-2}-\frac{1}{s+2}}-\frac{1}{s^2+4}}\]
    \[=\frac{1}{32}e^{2t}-\frac{1}{32}e^{-2t}-\frac{1}{16}\sin(2t)\]

    \item [g.)] \[\lpi\bracks{\frac{42}{(s-2)(s+4)(s+5)}}=\lpi\bracks{\frac{1}{s-2}-\frac{7}{s+4}+\frac{6}{s+5}}=e^{2t}-7e^{-4t}+6e^{-5t}\]
\end{itemize}
\end{document}
