\documentclass[12pt]{article}
\pagenumbering{gobble}
\linespread{1}

\usepackage{amsfonts}
\usepackage{amsmath}
\usepackage{amssymb}
\usepackage{array}
\usepackage{fancyhdr}
\usepackage{mathtools}
\usepackage{textcomp}
\usepackage[margin=1in,headheight=10mm]{geometry}

\newcommand{\contradiction}{%
    \ensuremath{{\Rightarrow\mspace{-2mu}\Leftarrow}}%
}

\newcommand{\angleb}[1]{\left\langle#1\right\rangle}
\newcommand{\vertb}[1]{\left\vert#1\right\vert}
\newcommand{\bracks}[1]{\left[#1\right]}
\newcommand{\parns}[1]{\left(#1\right)}
\newcommand{\dvert}[1]{\left\Vert#1\right\Vert}

\begin{document}
\pagestyle{fancy}
\fancyhead{}
\fancyhead[L]{Alexander Agruso}
\fancyhead[R]{MATH 2393 Homework 9}

\normalsize
\section*{Exercises 16.3}
\begin{itemize}
    \item [3.)] \[M_y=x+2y,\ne N_x=2x+2y\]
    Thus $F$ is not a conservative field.

    \item [7.)] \[M_y=2y\cos x-\sin y=N_x=2y\cos x-\sin y\]
    Thus $F$ is a conservative field.
    \[F=\nabla f\implies f=\int y^2\cos x+\cos y\,dx=y^2\sin x+x\cos y+C\]

    \item [13.)] \[f=\int x^2y^3\,dx=\frac{1}{3}x^3y^3+C\]
    \[I=\int_C\nabla f\,dr=f(r(1))-f(r(0))=-9-0=-9\]

    \item [19.)] \[M_y=-2xe^{-y}=N_x=-2xe^{-y}\]
    Thus $F$ is a conservative field.
    \[r(t)=\angleb{t+1,t}\]
    \[f=\int2xe^{-y}\,dx+\int2y\,dy=x^2e^{-y}+y^2+C\]
    \[\implies I=f(r(1))-f(r(0))=\frac{4}{e}+1-1=\frac{4}{e}\]

    \item [23.)] \[M_y=0=N_x=0\]
    \[r(t)=\angleb{t+1,2t}\]
    \[f=\int x^3\,dx+\int y^3\,dy=\frac{1}{4}x^4+\frac{1}{4}y^4\]
    \[\implies W=f(r(1))-f(r(0))=8-\frac{1}{4}=\frac{31}{4}\]
\end{itemize}
\section*{Exercises 16.4}
\begin{itemize}
    \item [1.)] \[I=\oint_Cy^2\,dx+x^2y\,dy=\int^5_0\int^4_02xy-2y\,dy\,dx=\int^5_0\bracks{xy^2-y^2}^4_0=16\int^5_0x-1\,dx\]
    \[=16\bracks{\frac{1}{2}x^2-x}^5_0=200-80=120\]

    \item [5.)] \[I=\oint_Cye^x\,dx+2e^x\,dy=\int^4_0\int^3_0e^x\,dx\,dy=\int^4_0e^3-1\,dy=\bracks{y(e^3-1)}^4_0=4(e^3-1)\]

    \item [7.)] \[I=\oint_Cy+e^{\sqrt x}\,dx+2x+\cos y^2\,dy=\int^1_0\int^{\sqrt x}_{x^2}\,dy\,dx=\int^1_0\sqrt{x}-x^2\,dx=\bracks{\frac{2}{3}x^{3/2}-\frac{1}{3}x^3}^1_0\]
    \[=\frac{2}{3}-\frac{1}{3}=\frac{1}{3}\]

    \item [11.)]
\end{itemize}
\end{document}
