\documentclass[12pt]{article}
\pagenumbering{gobble}
\linespread{1.25}

\usepackage{amsfonts}
\usepackage{amsmath}
\usepackage{amssymb}
\usepackage{array}
\usepackage{fancyhdr}
\usepackage{mathrsfs}
\usepackage{mathtools}
\usepackage{textcomp}
\usepackage[margin=1in,headheight=1in]{geometry}

\newcommand{\contradiction}{
    \ensuremath{{\Rightarrow\mspace{-2mu}\Leftarrow}}
}

% bracket commands
\newcommand{\angleb}[1]{\left\langle#1\right\rangle} % <>
\newcommand{\vertb}[1]{\left\vert#1\right\vert}      % ||
\newcommand{\bracks}[1]{\left[#1\right]}             % []
\newcommand{\braces}[1]{\left\{#1\right\}}           % {}
\newcommand{\parens}[1]{\left(#1\right)}             % ()

% set aliases
\newcommand{\N}{\mathbb{N}}
\newcommand{\Z}{\mathbb{Z}}
\newcommand{\Q}{\mathbb{Q}}
\newcommand{\R}{\mathbb{R}}

\newcommand{\derv}[2]{\dfrac{d#1}{d#2}}
\newcommand{\e}{\varepsilon}
\newcommand{\di}{\,/\,}

\newcommand{\lm}[1]{\displaystyle\lim_{#1}}

\begin{document}
\pagestyle{fancy}
\fancyhead{}
\fancyhead[L]{Alex Agruso}
\fancyhead[R]{Abstract Algebra Homework 2}

\normalsize

\section*{Chapter 1}
\begin{itemize}
    \item [5.)] awd

    \item [15.)] awd

\end{itemize}

\section*{Chapter 2}
\begin{itemize}
    \item [7.)] \begin{itemize}
        \item [1.] Let $a$ and $b$ be odd integers, thus there exist $m,n\in\Z$ where $a=2m+1$ and $b=2n+1$. We can see that $a+b=2m+1+2n+1=2m+2n+2=2(m+n+1)$, which is even, thus the odd integers are not closed under addition, and thus are not a group under addition.

        \item [2.] For the sake of establishing a contradiction, let $a$ and $b$ be odd integers where $a+b=a$, thus for some $m,n\in\Z$:
        \[2m+1+2n+1=2m+2n+2=2m+1\]
        \[\implies2n+1=0\implies2n=-1\implies n=-\frac{1}{2}\]
        Thus $n\notin\Z$.\contradiction Thus no such $a,b$ exist in the odd integers, thus the odd integers lack an identity element under addition, and thus are not a group under addition.
    \end{itemize}

    \item [14.)] \begin{itemize}
        \item [1.] $(ab)^3=(ab)(ab)(ab)=ababab$

        \item [2.] $(ab^{-2}c)^{-2}=(ab^{-2}c)^{-1}(ab^{-2}c)^{-1}=(c^{-1}b^2a^{-1})(c^{-1}b^2a^{-1})=c^{-1}b^2a^{-1}c^{-1}b^2a^{-1}$
    \end{itemize}

    \item [33.)] \[
        \begin{tabular}{l|lllll}
            & $e$ & $a$ & $b$ & $c$ & $d$ \\
            \hline
            $e$ & $e$ & $a$ & $b$ & $c$ & $d$ \\
            $a$ & $a$ & $b$ & $c$ & $d$ & $e$ \\
            $b$ & $b$ & $c$ & $d$ & $e$ & $a$ \\
            $c$ & $c$ & $d$ & $e$ & $a$ & $b$ \\
            $d$ & $d$ & $e$ & $a$ & $b$ & $c$
        \end{tabular}
        \]

\end{itemize}

\end{document}
