\documentclass[11pt]{article}
\pagenumbering{gobble}
\linespread{1.25}

\usepackage{amsfonts}
\usepackage{amsmath}
\usepackage{amssymb}
\usepackage{array}
\usepackage{fancyhdr}
\usepackage{mathrsfs}
\usepackage{mathtools}
\usepackage{textcomp}

\usepackage[margin=1in,headheight=1in]{geometry}

\newcommand{\contradiction}{
    \ensuremath{{\Rightarrow\mspace{-2mu}\Leftarrow}}
}

% bracket commands
\newcommand{\angleb}[1]{\left\langle#1\right\rangle} % <>
\newcommand{\vertb}[1]{\left\vert#1\right\vert}      % ||
\newcommand{\bracks}[1]{\left[#1\right]}             % []
\newcommand{\braces}[1]{\left\{#1\right\}}           % {}
\newcommand{\p}[1]{\left(#1\right)}             % ()

% set aliases
\newcommand{\N}{\mathbb{N}}
\newcommand{\Z}{\mathbb{Z}}
\newcommand{\Q}{\mathbb{Q}}
\newcommand{\R}{\mathbb{R}}
\newcommand{\C}{\mathbb{C}}

\newcommand{\derv}[2]{\dfrac{d#1}{d#2}}
\newcommand{\e}{\varepsilon}
\newcommand{\di}{\,/\,}

\newcommand{\lm}[1]{\displaystyle\lim_{#1}}

\begin{document}
\pagestyle{fancy}
\fancyhead{}
\fancyhead[L]{Alex Agruso}
\fancyhead[R]{Topology Extra Credit 2}

\normalsize

\begin{itemize}
    \item [a.)] Let $x\in S^3\subset\R^4$. Since $\R^4\cong\C^2$, we know that $(x_1,x_2,x_3,x_4)\mapsto(w_1,w_2)$ where $w_1,w_2\in\C$. Let $w_1=a+bi$ and $w_2=c+di$ for $a,b,c,d\in\R$. By definition of $S^3$, $x_1^2+x_2^2+x_3^2+x_4^2=1$, thus $a^2+b^2+c^2+d^2=1$. Consider $2w_1\overline{w_2}$ and $w_1\overline{w_1}-w_2\overline{w_2}$:
    \[2w_1\overline{w_2}=2(a+bi)(c-di)=2(ac+bci-adi+bd)=2(ac+bd)+2i(bc-ad)\]
    \[w_1\overline{w_1}-w_2\overline{w_2}=(a+bi)(a-bi)-(c+di)(c-di)=a^2+b^2-\p{c^2+d^2}\]
    Thus $2w_1\overline{w_2}\in\C$ and $(w_1\overline{w_1}-w_2\overline{w_2})\in\R$. Since $\C\times\R\cong\R^3$, we know that $(z,r)\mapsto y\in\R^3$. Let $y_1=2(ac+bd)$, $y_2=2(bc-ad)$, and $y_3=a^2+b^2-\p{c^2+d^2}$. Consider $y_1^2$, $y_2^2$, and $y_3^2$:
    \[y_1^2=2^2(ac+bd)^2=4\p{a^2c^2+2abcd+b^2d^2}\]
    \[y_2^2=2^2(bc-ad)^2=4\p{b^2c^2-2abcd+a^2d^2}\]
    \[y_3^2=\p{\p{a^2+b^2}-\p{c^2+d^2}}^2=\p{a^2+b^2}^2-2\p{a^2+b^2}\p{c^2+d^2}+\p{c^2+d^2}^2\]
    \[=\]

    \item [b.)] awd
    
    \item [c.)] awd
\end{itemize}


\end{document}
