\documentclass[12pt]{article}
\pagenumbering{gobble}

\usepackage{amsfonts}
\usepackage{amsmath}
\usepackage{amssymb}
\usepackage{array}
\usepackage{fancyhdr}
\usepackage{mathtools}
\usepackage{textcomp}
\usepackage[margin=1in,headheight=1in]{geometry}

\newcommand{\contradiction}{
    \ensuremath{{\Rightarrow\mspace{-2mu}\Leftarrow}}
}

\newcommand{\angleb}[1]{\left\langle#1\right\rangle}
\newcommand{\vertb}[1]{\left\vert#1\right\vert}
\newcommand{\bracks}[1]{\left[#1\right]}
\newcommand{\parns}[1]{\left(#1\right)}

\newcommand{\lp}{\mathcal{L}}
\newcommand{\lpi}{\mathcal{L}^{-1}}

\newcommand{\derv}[2]{\dfrac{d#1}{d#2}}
\newcommand{\pderv}[2]{\dfrac{\partial#1}{\partial#2}}

\begin{document}
\pagestyle{fancy}
\fancyhead{}
\fancyhead[L]{Alexander Agruso}
\fancyhead[R]{MATH 3323 Homework 18}

\normalsize
\begin{itemize}
    \item [a.)] \[\lpi\bracks{\frac{4}{s}}=4\]

    \item [b.)] \[\lpi\bracks{\frac{2}{s+3}}=2e^{-3t}\]

    \item [c.)] \[\lpi\bracks{\frac{2}{s^3}}=t^2\]

    \item [d.)] \[\lpi\bracks{\frac{s}{s^2+9}}=\cos(3t)\]

    \item [e.)] \[\lpi\bracks{\frac{4}{s^2+16}}=\sin(4t)\]

    \item [f.)] \[\lpi\bracks{\frac{s}{s^2-9}}=\lpi\bracks{\frac{s}{(s-3)(s+3)}}=\frac{1}{6}\lpi\bracks{\frac{3}{s+3}+\frac{3}{s-3}}=\frac{1}{2}e^{-3t}+\frac{1}{2}e^{3t}\]

    \item [g.)] \[\lpi\bracks{\frac{1}{s^2+4}}=\frac{1}{2}\lpi\bracks{\frac{2}{s^2+4}}=\frac{1}{2}\sin(2t)\]

    \item [h.)] \[\lpi\bracks{\frac{s-1}{(s^2-9)}}=\lpi\bracks{\frac{s-1}{(s-3)(s+3)}}=\lpi\bracks{\frac{s}{(s-3)(s+3)}-\frac{1}{(s-3)(s+3)}}\]
    \[=\frac{1}{6}\lpi\bracks{\frac{3}{s+3}+\frac{3}{s-3}-\frac{1}{s-3}+\frac{1}{s+3}}=\frac{1}{6}\lpi\bracks{\frac{4}{s+3}+\frac{2}{s-3}}=\frac{2}{3}e^{-3t}+\frac{1}{3}e^{3t}\]

\end{itemize}
\begin{itemize}
    \item [a.)] \[\lpi\bracks{\frac{s+3}{(s+3)^2+16}}=e^{-3t}\lpi\bracks{\frac{s}{s^2+16}}=e^{-3t}\cos(4t)\]

    \item [b.)] \[\lpi\bracks{\frac{1}{(s-2)^2+4}}=\frac{1}{2}e^{2t}\lpi\bracks{\frac{2}{s^2+4}}=\frac{1}{2}e^{2t}\sin(2t)\]

    \item [c.)] \[\lpi\bracks{\frac{1}{(s-4)^5}}=e^{4t}\lpi\bracks{\frac{1}{s^5}}=\frac{1}{24}e^{4t}\lpi\bracks{\frac{24}{s^5}}=\frac{1}{24}e^{4t}t^4\]

    \item [d.)] \[\lpi\bracks{\frac{s}{(s-4)^5}}=e^{4t}\lpi\bracks{\frac{s+4}{s^5}}=e^{4t}\lpi\bracks{\frac{1}{s^4}+\frac{4}{s^5}}=\frac{1}{6}e^{4t}\lpi\bracks{\frac{6}{s^4}+\frac{24}{s^5}}\]
    \[=\frac{1}{6}e^{4t}(t^3+t^4)\]

    \item [e.)] \[\lpi\bracks{\frac{s^2}{(s-4)^5}}=e^{4t}\lpi\bracks{\frac{(s+4)^2}{s^5}}=e^{4t}\lpi\bracks{\frac{s^2+8s+16}{s^5}}\]
    \[=e^{4t}\lpi\bracks{\frac{1}{s^3}+\frac{8}{s^4}+\frac{16}{s^5}}=e^{4t}\parns{\frac{1}{2}\lpi\bracks{\frac{2}{s^3}}+\frac{4}{3}\lpi\bracks{\frac{6}{s^4}}+\frac{2}{3}\lpi\bracks{\frac{24}{s^5}}}\]
    \[=e^{4t}\parns{\frac{1}{2}t^2+\frac{4}{3}t^3+\frac{2}{3}t^4}\]

    \item [f.)] \[\lpi\bracks{\frac{s+5}{(s+2)^2+16}}=e^{-2t}\lpi\bracks{\frac{s+3}{s^2+16}}=e^{-2t}\lpi\bracks{\frac{s}{s^2+16}+\frac{3}{s^2+16}}\]
    \[=e^{-2t}\parns{\cos(4t)+\frac{4}{3}\sin(4t)}\]

    \item [g.)] \[\lpi\bracks{\frac{s+3}{s^2+4s+13}}=\lpi\bracks{\frac{s+3}{(s+2)^2+9}}=e^{-2t}\lpi\bracks{\frac{s+1}{s^2+9}}\]
    \[=e^{-2t}\lpi\bracks{\frac{s}{s^2+9}+\frac{1}{s^2+9}}=e^{-2t}\parns{\cos(3t)+\frac{1}{3}\sin(3t)}\]

    \item [h.)] \[\lpi\bracks{\frac{s-4}{s^2-2s+7}}=\lpi\bracks{\frac{s-4}{(s-1)^2+6}}=e^t\lpi\bracks{\frac{s-3}{s^2+6}}\]
    \[=e^t\bracks{\cos\parns{\sqrt6 t}-\frac{3}{\sqrt6}\sin\parns{\sqrt6 t}}\]
\end{itemize}
\end{document}
