\documentclass[12pt]{article}
\pagenumbering{gobble}
\linespread{1.15}

\usepackage{amsfonts}
\usepackage{amsmath}
\usepackage{amssymb}
\usepackage{array}
\usepackage{fancyhdr}
\usepackage{textcomp}
\usepackage[margin=1in,headheight=1in]{geometry}

\newcommand{\contradiction}{
    \ensuremath{{\Rightarrow\mspace{-2mu}\Leftarrow}}
}

\newcommand{\angleb}[1]{\left\langle#1\right\rangle}
\newcommand{\vertb}[1]{\left\vert#1\right\vert}
\newcommand{\bracks}[1]{\left[#1\right]}

\newcommand{\derv}[2]{\dfrac{d#1}{d#2}}

\begin{document}
\pagestyle{fancy}
\fancyhead{}
\fancyhead[L]{Alexander Agruso}
\fancyhead[R]{MATH 3323 Homework 3}

\normalsize
\begin{itemize}
    \item [1.)] Manipulate to standard form:
    \begin{equation*}
        x^2\derv{y}{x}+x(x+2)y=x^2\derv{y}{x}+x^2y+2xy\implies \derv{y}{x}+y\left(1+\dfrac{2}{x}\right)=\dfrac{e^x}{x^2}
    \end{equation*}
    Find $\mu(x)$ then $y$:
    \begin{equation*}
        \mu(x)=e^{\int p(x)dx}=e^{\int1+\frac{2}{x}dx}=e^{x+2\ln\vert x\vert}=e^xe^{2\ln\vert x\vert}=e^xx^2
    \end{equation*}
    \begin{equation*}
        y=\dfrac{1}{\mu(x)}\int\mu(x)g(x)\ dx=\dfrac{1}{e^xx^2}\bracks{\int e^{2x}\ dx}=\dfrac{e^x}{2x^2}+\dfrac{C}{e^xx^2}
    \end{equation*}

    Which is the explicit solution.

    \item [2.)] Manipulate to standard form:
    \begin{equation*}
        \cos xdy+y\sin xdx-dx=0\implies \cos x\derv{y}{x}+y\sin x-1=0
    \end{equation*}
    \begin{equation*}
        \implies\derv{y}{x}+y\tan x=\sec x
    \end{equation*}
    Find $\mu(x)$ then $y$:
    \begin{equation*}
        \mu(x)=e^{\int\tan xdx}=e^{-\ln\vert\cos x\vert}=\sec x
    \end{equation*}
    \begin{equation*}
        y=\dfrac{1}{\sec x}\bracks{\int\sec^2x\ dx}=\dfrac{\tan x}{\sec x}+\dfrac{C}{\sec x}
    \end{equation*}
    Which is the explicit solution.

    \item [3.)] $y=\dfrac{\tan x}{\sec x}+\dfrac{C}{\sec x}$ as per problem 2.

    \item [4.)] Find $\mu(x)$ then $y$:
    \begin{equation*}
        \mu(x)=e^{\int \sin xdx}=e^{-\cos x}=\dfrac{1}{e^{\cos x}}
    \end{equation*}
    \begin{equation*}
        y=e^{\cos x}\bracks{\int\dfrac{e^{\cos x}}{e^{\cos x}}\ dx}=e^{\cos x}(x+C)
    \end{equation*}
    Solving given the initial values:
    \begin{equation*}
        -2.5=e^{\cos(0)}(0+C)=Ce^1\implies C=\dfrac{-2.5}{e}
    \end{equation*}
    \begin{equation*}
        \therefore y=e^{\cos x}\left(x+\dfrac{-2.5}{e}\right)
    \end{equation*}
    Which is the particular solution.

    \pagebreak
    \item [5.)] Manipulate to standard form:
    \begin{equation*}
        \derv{y}{x}=x-4xy\implies\derv{y}{x}+4xy=x
    \end{equation*}
    Find $\mu(x)$ then $y$:
    \begin{equation*}
        \mu(x)=e^{\int4xdx}=e^{2x^2}
    \end{equation*}
    \begin{equation*}
        y=\dfrac{1}{e^{2x^2}}\bracks{\int xe^{2x^2}\ dx}=\dfrac{1}{e^{2x^2}}\left(\dfrac{e^{2x^2}}{4}+C\right)=\dfrac{1}{4}+\dfrac{C}{e^{2x^2}}
    \end{equation*}
    Which is the explicit solution.

    \item [6.)] Find $\mu(t)$ then $y$:
    \[\mu(t)=e^{\int-dt}=e^{-t}\]
    \[y=e^t\bracks{\int2te^t\ dt}=e^t(2te^t-2e^t+C)=2te^{2t}-2e^{2t}+e^tC\]
    Solving given the initial values:
    \[1=2(0)e^{2(0)}-2e^{2(0)}+e^0C=C-2\implies C=3\]
    \[\therefore y=2te^{2t}-2e^{2t}+3e^t\]
    Which is the particular solution.

    \item [7.)] Manipulate to standard form:
    \[t\dfrac{dy}{dx}+(t+1)y=t\implies\dfrac{dy}{dx}+\left(\dfrac{t+1}{t}\right)y=1\]
    Find $\mu(t)$ then $y$:
    \[e^{\int\left(\frac{t+1}{t}\right)dt}=e^{t+\ln\vert t\vert}=te^t\]
    \[y=\dfrac{1}{te^t}\bracks{\int te^t\ dt}=\dfrac{1}{te^t}\left(te^t-e^t+C\right)=1-\dfrac{1}{t}+\dfrac{C}{te^t}\]
    Solving given the initial values:
    \[1=1-\dfrac{1}{\ln 2}+\dfrac{C}{\ln 2e^{\ln 2}}\implies\dfrac{1}{\ln 2}=\dfrac{C}{2\ln 2}\implies C=2\]
    \[\therefore y=1-\dfrac{1}{t}+\dfrac{1}{\ln 2}\]
    Which is the particular solution.

    \pagebreak
    \item [8.)] Find $\mu(x)$ then $y$:
    \[\mu(x)=e^{\int2dt}=e^{2t}\]
    \[y=\dfrac{1}{e^{2t}}\bracks{\int t\ dt}=\dfrac{1}{e^{2t}}\left(\dfrac{t^2}{2}+C\right)=\dfrac{t^2}{2e^{2t}}+\dfrac{C}{e^{2t}}\]
    Solving given the initial values:
    \[0=\dfrac{(1)^2}{2e^{2(1)}}+\dfrac{C}{e^{2(1)}}=\dfrac{1}{2e^2}+\dfrac{C}{e^2}\implies C=-\dfrac{1}{2}\]
    \[\therefore y=\dfrac{t^2}{2e^{2t}}-\dfrac{1}{2e^{2t}}=\dfrac{t^2-1}{2e^{2t}}\]
    Which is the particular solution.

\end{itemize}

\end{document}
