\documentclass[12pt]{article}
\pagenumbering{gobble}
\linespread{1}

\usepackage{amsfonts}
\usepackage{amsmath}
\usepackage{amssymb}
\usepackage{array}
\usepackage{fancyhdr}
\usepackage{mathtools}
\usepackage{textcomp}
\usepackage[margin=1in,headheight=10mm]{geometry}

\newcommand{\contradiction}{%
    \ensuremath{{\Rightarrow\mspace{-2mu}\Leftarrow}}%
}

\newcommand{\pderv}[2]{{\partial#1}/{\partial#2}}

\newcommand{\angleb}[1]{\left\langle#1\right\rangle}
\newcommand{\vertb}[1]{\left\vert#1\right\vert}
\newcommand{\bracks}[1]{\left[#1\right]}
\newcommand{\parns}[1]{\left(#1\right)}
\newcommand{\dvert}[1]{\left\Vert#1\right\Vert}

\begin{document}
\pagestyle{fancy}
\fancyhead{}
\fancyhead[L]{Alexander Agruso}
\fancyhead[R]{MATH 2393 Homework 6}

\normalsize
\section*{Exercises 15.1}
\begin{itemize}
    \item [15.)] \[\int^4_1\int^2_0\left(6x^2y-2x\right)\,dy\,dx=\int_{1}^{4}\bracks{3x^2y^2-2xy}^2_0\,dx=\int_{1}^{4}12x^2-4x\,dx\]
    \[=\bracks{4x^3-2x^2}^4_1=256-32-4+2=222\]

    \item [19.)] \[\int^3_{-3}\int^{\pi/2}_0(y+y^2\cos x)\,dx\,dy=\int^3_{-3}\bracks{xy+y^2\sin x}^{\pi/2}_0=\int^3_{-3}\frac{\pi}{2}y+y^2\,dy\]
    \[=\bracks{\frac{\pi}{4}y^2+\frac{y^3}{3}}^3_{-3}=\frac{9\pi}{4}+9-\frac{9\pi}{4}+9=18\]

    \item [29.)] \[\iint\limits_R\frac{xy^2}{x^2+1}\,dA=\int^3_{-3}\int^1_0\frac{xy^2}{x^2+1}\,dx\,dy=\frac{1}{2}\int^3_{-3}\int^1_0\frac{y^2}{u}\,du\,dy=\frac{1}{2}\int^3_{-3}\bracks{y^2\ln\vert u\vert}^1_0\]
    \[=\frac{1}{2}\int^3_{-3}\bracks{y^2\ln\vert x^2+1\vert}^1_0=\frac{1}{2}\int^3_{-3}\bracks{y^2\ln2}\,dy=\frac{\ln2}{2}\bracks{\frac{y^3}{3}}^3_{-3}=\frac{18\ln2}{2}=9\ln2\]

    \item [33.)] \[\iint\limits_Rye^{-xy}\,dA=\int^3_0\int^2_0ye^{-xy}\,dx\,dy=\int^3_0\bracks{-e^{-xy}dy}^2_0=\int^3_{0}-e^{-2y}+e^0\,dy\]
    \[\int^3_{0}1-e^{-2y}\,dy=\bracks{y+\frac{e^{-2y}}{2}}^3_0=3+\frac{e^{-6}}{2}-\frac{1}{2}=\frac{e^{-6}+5}{2}\]

    \item [41.)] Find the limits:
    \[-1\leq x\leq1,\ 0\leq y\leq1\]
    Evaluate the integral:
    \[\iint\limits_R1+x^2ye^y\,dA=\int^1_0\int^1_{-1}1+x^2ye^y\,dx\,dy=\int^1_0\bracks{x+\frac{1}{3}x^3ye^y}^1_{-1}\,dy\]
    \[=\int^1_01+\frac{1}{3}ye^y+1+\frac{1}{3}ye^y\,dy=\int^1_02+\frac{2}{3}ye^y\,dy=\bracks{2y+\frac{2}{3}\parns{ye^y-e^y}}^1_0\]
    \[=2+\frac{2}{3}=\frac{8}{3}\]

\end{itemize}

\section*{Exercises 15.2}
\begin{itemize}
    \item [3.)] \[\int^1_0\int^y_0xe^{y^3}\,dx\,dy=\int^1_0\bracks{\frac{x^2e^{y^3}}{2}}^y_0\,dy=\int^1_0\frac{y^2e^{y^3}}{2}\,dy=\frac{1}{6}\bracks{e^u}^1_0=\frac{1}{6}\bracks{e^{y^3}}^1_0=\frac{e-1}{6}\]

    \item [13.)] \[\iint\limits_Dx\,dA=\int^1_0\int^x_0x\,dy\,dx=\int^1_0\bracks{xy}^x_0\,dx=\int^1_0x^2\,dx=\bracks{\frac{x^3}{3}}^1_0=\frac{1}{3}\]
    \[\iint\limits_Dx\,dA=\int^1_0\int^1_yx\,dx\,dy=\int^1_0\bracks{\frac{x^2}{2}}^1_y\,dx=\int^1_0\frac{1}{2}-\frac{y^2}{2}\,dx=\bracks{\frac{y}{2}-\frac{y^3}{6}}^1_0=\frac{1}{2}-\frac{1}{6}=\frac{1}{3}\]

    \item [15.)] \[\iint\limits_Dy\,dA=\int^2_{-1}\int_{y^2}^{y+2}y\,dx\,dy=\int^2_{-1}\bracks{xy}^{y+2}_{y^2}=\int^2_{-1}2y+y^2-y^3\,dy\]
    \[=\bracks{y^2+\frac{y^3}{3}-\frac{y^4}{4}}^2_{-1}=4+\frac{8}{3}-\frac{16}{4}-1+\frac{1}{3}+\frac{1}{4}=3-1+\frac{1}{4}=\frac{9}{4}\]
    Integrating with respect to $x$ first is easier as it prevents us from having to evaluate two double integrals.

    \item [17.)] \[\iint\limits_Dx\cos y\,dA=\int^1_0\int^{x^2}_0x\cos y\,dy\,dx=-\int^1_0\bracks{x\sin y}^{x^2}_0\,dx=-\int^1_0x\sin x^2\,dx\]
    \[=-\frac{1}{2}\int^1_0\sin u\,du=-\frac{1}{2}\bracks{\cos u}^1_0=-\frac{1}{2}(\cos(1)-1)=\frac{1-\cos(1)}{2}\]

    \item [23.)] \[\iint\limits_D3x+2y\,dy\,dx=\int^1_0\int^{\sqrt x}_{x^2}3x+2y\,dy\,dx=\int^1_0\bracks{3xy+y^2}^{\sqrt x}_{x^2}\,dx\]\[=\int^1_03x^{3/2}+x-3x^3-x^4\,dx=\bracks{\frac{6x^{5/2}}{5}+\frac{x^2}{2}-\frac{3x^4}{4}-\frac{x^5}{5}}=\frac{6}{5}+\frac{1}{2}-\frac{3}{4}-\frac{1}{5}=1-\frac{1}{4}=\frac{3}{4}\]

    \pagebreak
    \item [45.)] \[\int^1_0\int^y_0f(x,y)\,dx\,dy=\int^1_0\int^1_xf(x,y)\,dy\,dx\]

    \item [53.)] \[\int^1_0\int^1_{\sqrt x}\sqrt{y^3+1}\,dy\,dx=\int^1_0\int^{y^2}_0\sqrt{y^3+1}\,dx\,dy=\int^1_0\bracks{x\sqrt{y^3+1}}^{y^2}_0\,dy\]
    \[=\int^1_0y^2\sqrt{y^3+1}\,dy=\frac{1}{3}\int^1_0\sqrt{u}\,du=\frac{1}{3}\bracks{\frac{2\sqrt{u^3}}{3}}^1_0=\frac{1}{3}\bracks{\frac{2\sqrt{\parns{y^3+1}^3}}{3}}^1_0=\]
    \[\frac{1}{3}\bracks{\frac{2\sqrt8-2}{3}}=\frac{2\parns{\sqrt8-1}}{9}\]

    \item [61.)] Find area of region of integration:
    \[A=\frac{1}{2}bh=\frac{1}{2}(1)(3)=\frac{3}{2}\]
    Now evaluate the integral:
    \[I=\int^1_0\int^{3x}_0xy\,dy\,dx=\int^1_0\bracks{\frac{xy^2}{2}}^{3x}_0\,dx=\int^1_0\frac{9x^3}{2}\,dx=\bracks{\frac{9x^3}{8}}^1_0=\frac{9}{8}\]
    Finally, evaluate $I/A$:
    \[I/A=\frac{9}{8}\times\frac{2}{3}=\frac{18}{24}=\frac{3}{4}\]

\end{itemize}

\section*{Exercises 15.3}
\begin{itemize}
    \item [5.)] \[\int^{3\pi/4}_{\pi/4}\int^2_1r\,dr\,d\theta=\int^{3\pi/4}_{\pi/4}\bracks{\frac{r^2}{2}}^2_1\,d\theta=\int^{3\pi/4}_{\pi/4}\frac{3}{2}\,d\theta=\frac{3}{2}\bracks{\theta}^{3\pi/4}_{\pi/4}=\frac{3\pi}{4}\]

    \item [7.)] Given $x=r\cos\theta$, $y=r\sin\theta$, and $J[x,y]=r$,
    \[f(x,y)=Jx^2y=r(r^2\cos^2\theta)(r\sin\theta)=r^4\cos^2\theta\sin\theta\]
    Evaluate the following integral:
    \[\iint\limits_{R}x^2y\,dA=\int^{\pi}_0\int^5_0r^4\cos^2\theta\sin\theta\,dr\,d\theta=\int^\pi_0\bracks{\frac{1}{5}r^5\cos^2\theta\sin\theta}^5_0\,d\theta\]
    \[625\int^\pi_0\cos^2\theta\sin\theta\,d\theta=-625\bracks{\frac{1}{3}\cos^3\theta}^\pi_0=625\cdot\frac{2}{3}=\frac{1250}{3}\]

    \item [19.)] \[I=\int^{2\pi}_0\int^5_0r^3\,dr\,d\theta=\int^{2\pi}_0\bracks{\frac{1}{4}r^4}^5_0\,d\theta=\frac{625}{4}\int^{2\pi}_0\,d\theta=\frac{1250\pi}{4}=\frac{625\pi}{2}\]

    \item [29.)] \[I=\int^{\pi/2}_0\int^2_0re^{-r^2}\,dr\,d\theta=-\frac{1}{2}\int^{\pi/2}_0\bracks{e^{-r^2}}^2_0=-\frac{1}{2}\int^{\pi/2}_0e^{-4}-1\,d\theta=\frac{\pi(1-e^{-4})}{4}\]

\end{itemize}
\section*{Exercises 15.4}
\begin{itemize}
    \item [17.)] \[I_x=\int^3_1\int^4_1y^4k\,dy\,dx=\int^3_1\bracks{\frac{1}{5}y^5k}^4_1\,dx=\int^3_1\parns{\frac{1023}{5}k}\,dx\]
    \[\frac{1023}{5}\bracks{xk}^3_1=\frac{2(1023)}{5}k=409.2k\]
    \[I_y=\int^3_1\int^4_1x^2ky^2\,dy\,dx=\int^3_1\bracks{\frac{1}{3}x^2ky^3}^4_1\,dx=\int^3_121x^2k\,dx\]
    \[=7\bracks{x^3k}^3_1=7(27k-1k)=7(26k)=182k\]
    \[I_0=\int^3_1\int^4_1(x^2+y^2)ky^2\,dy\,dx=I_x+I_y=591.2k\]

\end{itemize}
\section*{Exercises 15.9}
\begin{itemize}
    \item [1.)] \[J=\begin{vmatrix*}[r]
        2 & 1 \\
        4 & -1
    \end{vmatrix*}=-2-4=-6\]

    \item [3.)] \[J=\begin{vmatrix}
        \cos t & -s\sin t \\
        \sin t & s\cos t
    \end{vmatrix}=s\cos^2t+s\sin^2t=s\]

    \item [15.)] Given the triangle \{(0,0),(1,2),(2,1)\}, the transformation $x=2u+v$ and $y=u+2v$, and $J[u,v]=3$, we can evaluate the following integral:
    \[I=\iint\limits_{R}x-3y\,dA=3\int^1_0\int^{1-v}_0-u-5v\,du\,dv=3\int^1_0\bracks{-\frac{1}{2}u^2-5uv}^{1-v}_0\,dv\]
    \[=3\int^1_0-\frac{1}{2}(1-v)^2-5(1-v)v\,dv=\frac{3}{2}\int^1_09v^2-8v-1\,dv=\frac{3}{2}\bracks{3v^3-4v^2-v}^1_0\]
    \[=\frac{3}{2}\parns{3-4-1}=-3\]

    \item [17.)] Given the ellipse $9x^2+4y^2=36$, and applying the transformation $x=2u$ and $y=3v$, we get $u^2+v^2=1$ and $J[u,v]=6$. Converting to polar coordinates, we find $0\leq r\leq 1$, $0\leq\theta\leq2\pi$ and $J[r,\theta]=r$. Evaluating the following integral:
    \[I=\iint\limits_{R}x^2\,dA=6\int^{2\pi}_0\int^1_04r^3\cos^2\theta\,dr\,d\theta=6\int^{2\pi}_0\bracks{r^4\cos^2\theta}^1_0\,d\theta\]
    \[=6\int^{2\pi}_0\cos^2\theta\,d\theta=3\int^{2\pi}_01+\cos2\theta\,d\theta=3\bracks{\theta+\frac{1}{2}\sin2\theta}^{2\pi}_0=3\parns{2\pi+0+0+0}=6\pi\]

\end{itemize}
\end{document}
