\documentclass[12pt]{article}
\pagenumbering{gobble}

\usepackage{amsfonts}
\usepackage{amsmath}
\usepackage{amssymb}
\usepackage{array}
\usepackage{fancyhdr}
\usepackage{mathtools}
\usepackage{textcomp}
\usepackage{tikz}

\usepackage{pgfplots}
\pgfplotsset{compat=1.9}

\usetikzlibrary{math}

\usepackage[margin=1in,headheight=1in]{geometry}

\newcommand{\contradiction}{
    \ensuremath{{\Rightarrow\mspace{-2mu}\Leftarrow}}
}

\newcommand{\angleb}[1]{\left\langle#1\right\rangle}
\newcommand{\vertb}[1]{\left\vert#1\right\vert}
\newcommand{\bracks}[1]{\left[#1\right]}
\newcommand{\parns}[1]{\left(#1\right)}

\newcommand{\lp}{\mathcal{L}}
\newcommand{\lpi}{\mathcal{L}^{-1}}

\newcommand{\derv}[2]{\dfrac{d#1}{d#2}}
\newcommand{\pderv}[2]{\dfrac{\partial#1}{\partial#2}}

\begin{document}
\pagestyle{fancy}
\fancyhead{}
\fancyhead[L]{Alexander Agruso}
\fancyhead[R]{MATH 3323 Homework 20}

\normalsize
\begin{itemize}
    \item [1.)] \[y'-3y=e^{4t}\implies\lp\bracks{y'-3y}=\lp\bracks{e^{4t}}\implies sY(s)-y(0)-3Y(s)=\frac{1}{s-4}\]
    \[\implies (s-3)Y(s)=\frac{1}{s-4}\implies Y(s)=\frac{1}{(s-3)(s-4)}\]
    \[\implies y(t)=\lpi\bracks{\frac{1}{(s-3)(s-4)}}=-\lpi\bracks{\frac{1}{s-3}-\frac{1}{s-4}}=e^{4t}-e^{3t}\]

    \item [3.)] \[y''+4y'+4y=t^4e^{-2t}\implies\lp\bracks{y''+4y'+4y}=\lp\bracks{t^4e^{-2t}}\]
    \[\implies s^2Y(s)-s y(0)-y'(0)+4(sY(s)-y(0))+4Y(s)=\frac{24}{(s+2)^5}\]
    \[\implies (s+2)^2Y(s)-s-6=\frac{24}{(s+2)^5}\implies Y(s)=\frac{24}{(s+2)^7}+\frac{s}{(s+2)^2}-\frac{6}{(s+2)^2}\]
    \[\implies y(t)=\lpi\bracks{\frac{24}{(s+2)^7}}+\lpi\bracks{\frac{s}{(s+2)^2}}+\lpi\bracks{\frac{6}{(s+2)^2}}\]
    \[=\frac{1}{30}t^6e^{-2t}+\lpi\bracks{\frac{1}{s+2}-\frac{2}{(s+2)^2}}+6te^{-2t}=\frac{1}{30}t^6e^{-2t}+(1+4t)e^{-2t}\]

    \item [5.)] \[y''+y=(t-2)u_2(t)\implies\lp\bracks{y''+y}=\lp\bracks{(t-2)u_2(t)}\implies s^2Y(s)+Y(s)=\frac{e^{-2s}}{s^2}\]
    \[\implies (s^2+1)Y(s)=\frac{e^{-2s}}{s^2}\implies Y(s)=\frac{e^{-2s}}{s^2(s^2+1)}\implies y(t)=\lpi\bracks{\frac{e^{-2s}}{s^2(s^2+1)}}\]
    \[\lpi\bracks{\frac{1}{s^2(s^2+1)}}=\lpi\bracks{\frac{1}{s^2}-\frac{1}{s^2+1}}=t-\sin t\]
    \[\therefore\,y(t)=u_2(t)[(t-2)-\sin(t-2)]\]

\end{itemize}
\end{document}
