\documentclass[12pt]{article}
\pagenumbering{gobble}
\linespread{1}

\usepackage{amsfonts}
\usepackage{amsmath}
\usepackage{amssymb}
\usepackage{array}
\usepackage{fancyhdr}
\usepackage{textcomp}
\usepackage{pgfplots}
\usepackage[margin=1in,headheight=10mm]{geometry}

\usetikzlibrary{fillbetween}

\pgfplotsset{compat=1.17}

\newcommand{\contradiction}{%
    \ensuremath{{\Rightarrow\mspace{-2mu}\Leftarrow}}%
}

\newcommand{\angleb}[1]{\left\langle#1\right\rangle}
\newcommand{\vertb}[1]{\left\vert#1\right\vert}
\newcommand{\bracks}[1]{\left[#1\right]}
\newcommand{\parns}[1]{\left(#1\right)}
\newcommand{\dvert}[1]{\left\Vert#1\right\Vert}

\begin{document}
\pagestyle{fancy}
\fancyhead{}
\fancyhead[L]{Alexander Agruso}
\fancyhead[R]{MATH 2393 Homework 3}

\normalsize
\section*{Exercises 13.1}
\begin{itemize}
    \item [5.)] \[\lim_{t\to\infty}\angleb{
              \frac{1+t^2}{1-t^2},\tan^{-1}t,\frac{1-e^{-2t}}{t}}=\angleb{\lim_{t\to\infty}\frac{1+t^2}{1-t^2},\lim_{t\to\infty}\tan^{-1}t,\lim_{t\to\infty}\frac{1-e^{-2t}}{t}}\]
          \[\lim_{t\to\infty}\frac{1+t^2}{1-t^2}=\lim_{t\to\infty}\frac{2t}{-2t}=\lim_{t\to\infty}\frac{2}{-2}=-1\]
          \[\lim_{t\to\infty}\tan^{-1}t=\frac{\pi}{2}\]
          \[\lim_{t\to\infty}\frac{1-e^{-2t}}{t}=\lim_{t\to\infty}2e^{-2t}=\lim_{t\to\infty}\frac{2}{e^{2t}}=0\]
          \[\therefore\ \lim_{t\to\infty}\angleb{
              \frac{1+t^2}{1-t^2},\tan^{-1}t,\frac{1-e^{-2t}}{t}}=\angleb{-1,\frac{\pi}{2},0}\]
\end{itemize}
\section*{Exercises 13.2}
\begin{itemize}
    \item [11.)] \[\frac{d}{dt}\angleb{t^2,\cos(t^2),\sin^2t}=\angleb{2t,-2t\sin(t^2),2\sin t\cos t}\]

    \item [17.)] \[T(t)=\frac{r'(t)}{\Vert r'(t)\Vert}\]
          \[r'(t)=\angleb{2t-2,3,t^2+t}\]
          \[\Vert r'(t)\Vert=\sqrt{(2t-2)^2+3^2+(t^2+t)^2}=\sqrt{4t^2-8t+4+9+t^4+2t^3+t^2}\]
          \[=\sqrt{t^4+2t^3+5t^2-8t+13}\]
          \[\therefore\ T(t)=\frac{1}{\sqrt{t^4+2t^3+5t^2-8t+13}}\angleb{2t-2,3,t^2+t}\]
          \[T(2)=\angleb{\frac{2}{7},\frac{3}{7},\frac{6}{7}}\]

    \item [23.)] ***

    \item [35.)] \[\int_0^2(t\hat\imath-t^3\hat\jmath+3t^5\hat{k})\ dt=\left[\frac{t^2}{2}\hat\imath-\frac{t^4}{4}\hat\jmath+\frac{t^6}{2}\hat{k}\right]_0^2=2i-4j+32k\]

    \item [39.)] \[\int(\sec^2t\hat\imath+t(t^2+1)^3\hat\jmath+t^2\ln t\hat{k})\ dt\]
          \[\int\sec^2t\hat\imath\ dt=\tan t\hat\imath\]
          \[\int t(t^2+1)^3\hat\jmath\ dt=\frac{(t^2+1)^4}{8}\hat\jmath\]
          \[\int t^2\ln t\hat{k}\ dt=\left(\frac{t^3}{3}\ln t-\int\frac{t^3}{3t}\right)\hat{k}=\left(\frac{t^3\ln t}{3}-\frac{t^3}{9}\right)\hat{k}\]
          \[\therefore\ I=\tan t\hat\imath+\frac{(t^2+1)^4}{8}\hat\jmath+\left(\frac{t^3\ln t}{3}-\frac{t^3}{9}\right)\hat{k}+C\]

    \item [41.)] \[r(t)=\int r'(t)\ dt=t^2\hat\imath+t^3\hat\jmath+\frac{2\sqrt{t^3}}{3}\hat{k}+C\]
          \[\hat\imath+\hat\jmath=\hat\imath+\hat\jmath+\frac{2}{3}\hat{k}+C\implies C=-\frac{2}{3}\hat{k}\]
          \[\therefore\ r(t)=t^2\hat\imath+t^3\hat\jmath+\left(\frac{2\left(\sqrt{t^3}-1\right)}{3}\right)\hat{k}\]
\end{itemize}
\section*{Exercises 13.3}
\begin{itemize}
    \item [1.)] \[\int_{-5}^{5}\Vert r'(t)\Vert\ dt=\int_{-5}^{5}\Vert\angleb{1,-3\sin t,3\cos t}\Vert\ dt=\int_{-5}^{5}\sqrt{1^2+(-3\sin t)^2+(3\cos t)^2}\ dt\]
          \[=\int_{-5}^{5}\sqrt{1+9\sin^2t+9\cos^2t}\ dt=\int_{-5}^{5}\sqrt{1+9}\ dt=\int_{-5}^{5}\sqrt{10}\ dt=\bracks{\sqrt{10}t}_{-5}^5\]
          \[=5\sqrt{10}-(-5\sqrt{10})=10\sqrt{10}\]

    \item [17.)] \begin{itemize}
              \item [a.)]
                    \[T=\frac{r'}{\Vert r'\Vert}=\frac{\angleb{1,-3\sin t,3\cos t}}{\sqrt{1^2+(-3\sin t)^2+(3\cos t)^2}}=\frac{\angleb{1,-3\sin t,3\cos t}}{\sqrt{1+9\sin^2t+9\cos^2t}}\]
                    \[=\frac{\angleb{1,-3\sin t,3\cos t}}{\sqrt{1+9}}=\frac{1}{\sqrt{10}}\angleb{1,-3\sin t,3\cos t}\]
                    \[=\angleb{\frac{1}{\sqrt{10}},-\frac{3}{\sqrt{10}}\sin t,\frac{3}{\sqrt{10}}\cos t}\]
                    \[N=\frac{T'}{\Vert T'\Vert}=\frac{\angleb{0,-\frac{3}{\sqrt{10}}\cos t,-\frac{3}{\sqrt{10}}\sin t}}{\sqrt{0^2+\left(-\frac{3}{\sqrt{10}}\cos t\right)^2+\parns{-\frac{3}{\sqrt{10}}\sin t}^2}}=\frac{\angleb{0,-\frac{3}{\sqrt{10}}\cos t,-\frac{3}{\sqrt{10}}\sin t}}{\sqrt{\frac{9}{10}\cos^2t+\frac{9}{10}\sin^2t}}\]
                    \[=\frac{1}{\sqrt{\frac{9}{10}}}\angleb{0,-\frac{3}{\sqrt{10}}\cos t,-\frac{3}{\sqrt{10}}\sin t}=\angleb{0,-\frac{3}{3}\cos t,-\frac{3}{3}\sin t}\]
                    \[=\angleb{0,-\cos t,-\sin t}\]

              \item [b.)] \[\kappa=\frac{\Vert T'\Vert}{\Vert r'\Vert}=\frac{\frac{\sqrt{9}}{\sqrt{10}}}{\sqrt{10}}=\frac{\sqrt{9}}{10}=\frac{3}{10}\]
          \end{itemize}

    \item [21.)] \[r'=\angleb{0,3t^2,2t},\ r''=\angleb{0,6t,2}\]
          \[r'\times r''=\begin{vmatrix}
                  \hat\imath & \hat\jmath & \hat{k} \\
                  0       & 3t^2    & 2t      \\0 & 6t & 2
              \end{vmatrix}=(6t^2-12t^2)\hat\imath+0\hat\jmath+0\hat{k}=\angleb{-6t^2,0,0}\]
          \[\Vert r'\times r''\Vert=\sqrt{(-6t^2)^2+0^2+0^2}=\sqrt{36t^4}=6t^2\]
          \[\Vert r'\Vert^3=\parns{\sqrt{0^2+(3t^2)^2+(2t)^2}}^3=\parns{\sqrt{9t^4+4t^2}}^3=\parns{9t^4+4t^2}^{\frac{3}{2}}\]
          \[\therefore\ \kappa=\frac{6t^2}{\parns{9t^4+4t^2}^{\frac{3}{2}}}\]

    \item [47.)] \[T=\frac{r'}{\Vert r'\Vert}=\frac{\angleb{2t,2t^2,1}}{\sqrt{(2t)^2+(2t^2)^2+1^2}}=\frac{\angleb{2t,2t^2,1}}{\sqrt{4t^2+4t^4+1}}=\frac{\angleb{2t,2t^2,1}}{\sqrt{(2t^2+1)^2}}\]
    \[=\frac{\angleb{2t,2t^2,1}}{2t^2+1}=\angleb{\frac{2t}{2t^2+1},\frac{2t^2}{2t^2+1},\frac{1}{2t^2+1}}\]
    \[T\parns{1,\frac{2}{3},1}=\angleb{\frac{2(1)}{2(1)^2+1},\frac{2(2/3)^2}{2(2/3)^2+1},\frac{1}{2(1)^2+1}}=\angleb{\frac{2}{3},\frac{8}{17},\frac{1}{3}}\]
    \[N=\frac{T'}{\Vert T'\Vert}=\frac{\angleb{\frac{2-4t^2}{(2t^2+1)^2},\frac{2t^2}{(2t^2+1)^2},-\frac{4t}{(2t^2+1)^2}}}{\sqrt{\parns{\frac{2-4t^2}{(2t^2+1)^2}}^2+\parns{\frac{2t^2}{(2t^2+1)^2}}^2+\parns{-\frac{4t}{(2t^2+1)^2}}^2}}\]
    \[=\angleb{ }\]

\end{itemize}
\section*{Exercises 13.4}
\begin{itemize}
    \item [5.)] \[v(t)=r'(t)=\angleb{-3\sin t,2\cos t}\]
    \[a(t)=r''(t)=\angleb{-3\cos t,-2\sin t}\]
    \[\Vert v(t)\Vert=\Vert r'(t)\Vert=\sqrt{(-3\sin t)^2+(2\cos t)^2}=\sqrt{9\sin^2t+4\cos^2t}=\sqrt{5\sin^2t+4}\]

    \item [15.)] \[v(t)=\int a(t)\ dt=2t\hat\imath+t^2\hat{k}+C_1\]
    \[v(0)=3\hat\imath-\hat\jmath=2(0)\hat\imath+(0)^2\hat{k}+C_1=C_1\implies C_1=3\hat\imath-\hat\jmath\]
    \[\therefore\ v(t)=2t\hat\imath+t^2\hat{k}+3\hat\imath-\hat\jmath=(2t+3)\hat\imath-\hat\jmath+t^2\hat{k}\]
    \[r(t)=\int v(t)\ dt=(t^2+3t)\hat\imath-t\hat\jmath+\frac{t^3}{3}\hat{k}+C_2\]
    \[r(0)=\hat\jmath+\hat{k}=((0)^2+3(0))\hat\imath-(0)\hat\jmath+\frac{(0)^3}{3}\hat{k}+C_2=C_2\implies C_2=\hat\jmath+\hat{k}\]
    \[\therefore\ r(t)=(t^2+3t)\hat\imath-t\hat\jmath+\frac{t^3}{3}\hat{k}+\hat\jmath+\hat{k}=(t^2+3t)\hat\imath+(1-t)\hat\jmath+\left(\frac{t^3}{3}+1\right)\hat{k}\]

    \item [23.)] Establish initial variables and find $r(t)$:
\[v_0=200,\alpha=60^\circ,g=9.8\]
    \[\therefore\ r(t)=(200\cos(60^\circ))t\hat\imath+\bracks{(200\sin(60^\circ))t-\frac{gt^2}{2}}\hat\jmath=100t\hat\imath+\bracks{100\sqrt{3}t-\frac{9.8t^2}{2}}\hat\jmath\]
    Calculating the $x$-component of $r(t)$ at $t=\dfrac{2v_0\sin\alpha}{g}$ we can find the range:
    \[\text{range}=100\parns{\frac{2v_0\sin\alpha}{g}}=\frac{20000\sqrt{3}}{9.8}\approx3534.80\text{m}\]
    Calculating the $y$-component of $r(t)$ at $t$ such that the $y$-component of $r'(t)=0$, we can find the maximum height:
    \[\bracks{100\sqrt{3}-9.8t}=0\implies t=\frac{100\sqrt{3}}{9.8}\]
    \[\therefore\ \text{max height}=100\sqrt{3}t-\frac{9.8t^2}{2}\approx1530.61\text{m}\]
    To find $t$ at impact, we solve for $t>0$ when $y=0$:
    \[100\sqrt{3}t-\frac{9.8t^2}{2}=100\sqrt{3}t-4.9t^2=0\implies t=\frac{-100\sqrt{3}-\sqrt{30000}}{-9.8}=35.34\]
    \[\therefore\ \text{impact speed}=\Vert r'(t)\Vert=\sqrt{100^2+\parns{100\sqrt{3}-9.8t}^2}=200\text{m/s}\]

    \item [27.)] Solve for $y_{max}$:
    \[\frac{d}{dt}\bracks{(v_0\sin\alpha)t-\frac{1}{2}gt^2}=v_0\sin\alpha-gt=0\implies t=\frac{v_0\sin\alpha}{g}\]
    \[\therefore\ y_{max}=r_y\parns{\frac{v_0\sin\alpha}{g}}=(v_0\sin\alpha)\parns{\frac{v_0\sin\alpha}{g}}-\frac{1}{2}g\parns{\frac{v_0\sin\alpha}{g}}^2\]
    \[=\frac{v_0^2\sin^2\alpha}{g}-\frac{gv_0^2\sin^2\alpha}{2g^2}=\frac{2v_0^2\sin^2\alpha-v^2_0\sin^2\alpha}{2g}=\frac{v_0^2\sin^2\alpha}{2g}\]
    \[\implies 2gy_{max}=v_0^2\sin^2\alpha\implies v_0=\sqrt{\frac{2gy_{max}}{\sin^2\alpha}}=\frac{\sqrt{2gy_{max}}}{\sin\alpha}\]
    Finding our initial values:
    \[y_{max}=1600\text{ft},\ g=9.8\text{m/s}=32.144\text{ft/s}\]
    \[\therefore\ v_0=\frac{\sqrt{2(32.144)(1600)}}{\sin(36^\circ)}\approx545.64\text{ft/s}\]

\end{itemize}

\end{document}
