\documentclass[12pt]{article}
\pagenumbering{gobble}
\linespread{1}

\usepackage{amsfonts}
\usepackage{amsmath}
\usepackage{amssymb}
\usepackage{array}
\usepackage{fancyhdr}
\usepackage{mathtools}
\usepackage{textcomp}
\usepackage[margin=1in,headheight=10mm]{geometry}

\newcommand{\contradiction}{%
    \ensuremath{{\Rightarrow\mspace{-2mu}\Leftarrow}}%
}

\newcommand{\angleb}[1]{\left\langle#1\right\rangle}
\newcommand{\vertb}[1]{\left\vert#1\right\vert}
\newcommand{\bracks}[1]{\left[#1\right]}
\newcommand{\parns}[1]{\left(#1\right)}
\newcommand{\dvert}[1]{\left\Vert#1\right\Vert}

\begin{document}
\pagestyle{fancy}
\fancyhead{}
\fancyhead[L]{Alexander Agruso}
\fancyhead[R]{MATH 2393 Homework 7}

\normalsize
\section*{Exercises 15.6}
\begin{itemize}
    \item [3.)] \[I=\int^2_0\int^{z^2}_0\int^{y-z}_0(2x-y)\,dx\,dy\,dz=\int^2_0\int^{z^2}_0\bracks{x^2-xy}^{y-z}_0\,dy\,dz\]
    \[=\int^2_0\int^{z^2}_0(y-z)^2-(y-z)y\,dy\,dz=\int^2_0\int^{z^2}_0y^2-2yz+z^2-y^2+yz\,dy\,dz\]
    \[=\int^2_0\int^{z^2}_0z^2-yz\,dy\,dz=\int^2_0\bracks{yz^2-\frac{1}{2}y^2z}^{z^2}_0=\int^2_0z^4-\frac{1}{2}z^5\,dz\]
    \[=\bracks{\frac{1}{5}z^5-\frac{1}{12}z^6}^2_0=\frac{32}{5}-\frac{64}{12}=\frac{384}{60}-\frac{320}{60}=\frac{64}{60}=\frac{16}{15}\]

    \item [7.)] \[\int^\pi_0\int^1_0\int^{\sqrt{1-z^2}}_0z\sin x\,dy\,dz\,dx=\int^\pi_0\int^1_0\bracks{yz\sin x}^{\sqrt{1-z^2}}_0\,dz\,dx\]
    \[=\int^\pi_0\int^1_0z\sqrt{1-z^2}\sin x\,dz\,dx=-\frac{1}{2}\int^\pi_0\int^1_0\sqrt u\sin x\,du\,dx\]
    \[=-\frac{1}{2}\int^\pi_0\bracks{\frac{2}{3}\sqrt{(1-z^2)^3}\sin x}^1_0=\frac{1}{3}\int^\pi_0\sin x\,dx=\bracks{-\frac{1}{3}\cos x}^\pi_0=\frac{1}{3}+\frac{1}{3}=\frac{2}{3}\]

    \item [11.)] \[I=\int^4_1\int^4_y\int^z_0\frac{z}{x^2+z^2}\,dx\,dz\,dy=\int^4_1\int^4_y\bracks{\tan^{-1}\parns{\frac{x}{z}}}^z_0\,dz\,dy=\frac{\pi}{4}\int^4_1\int^4_y\,dz\,dy\]
    \[=\frac\pi4\int^4_1\bracks{z}^4_y\,dy=\frac{\pi}{4}\int^4_14-y\,dy=\frac\pi4\bracks{4y-\frac{1}{2}y^2}^4_1=\frac\pi4\parns{16-8-4+\frac{1}{2}}=\frac{9\pi}{8}\]

    \item [19.)] First, find bounds for $z$:
    \[2x+y+z=4\implies0\leq z\leq 4-2x-y\]
    Then find bounds for $x$ and $y$:
    \[2(0)+y+0=y=4\]
    \[2x+0+0=2x=4\implies x=2\]
    Thus the triangular region is bounded by the first quadrant and $y=4-2x$, thus
    \[0\leq x\leq2,\,0\leq y\leq4-2x\]
    Evaluate the integral:
    \[I=\int^2_0\int^{4-2x}_0\int^{4-2x-y}_0\,dz\,dy\,dx=\int^2_0\int^{4-2x}_04-2x-y\,dy\,dx\]
    \[=\int^2_0\bracks{4y-2xy-\frac{1}{2}y^2}^{4-2x}_0\,dx=\int^2_0-8x+16+4x^2-8x-\frac{1}{2}(4x^2-16x+16)\,dx\]
    \[=\int^2_02x^2-8x+8\,dx=\bracks{\frac{2}{3}x^3-4x^2+8x}^2_0=\frac{16}{3}-16+16=\frac{16}{3}\]

    \item [21.)] First, find bounds for $z$:
    \[x+y=1\implies0\leq z\leq1-y\]
    Then find bounds for $x$ and $y$:
    \[z=0\implies y=1\implies 1=x^2\implies x=\pm1\]
    Thus
    \[-1\leq x\leq1,\,x^2\leq y\leq1\]
    Evaluate the integral:
    \[\int^1_{-1}\int^1_{x^2}\int^{1-y}_0\,dz\,dy\,dx=\int^1_{-1}\int^1_{x^2}1-y\,dy\,dx=\int^1_{-1}\bracks{y-\frac{1}{2}y^2}^1_{x^2}\,dx\]
    \[=\int^1_{-1}\frac{1}{2}-x^2+\frac{1}{2}x^4\,dx=\bracks{\frac{1}{2}x-\frac{1}{3}x^3+\frac{1}{10}x^5}^1_{-1}=\frac{1}{2}-\frac{1}{3}+\frac{1}{10}+\frac{1}{2}-\frac{1}{3}+\frac{1}{10}=\frac{8}{15}\]

    \item [54.)] \[I=\]

\end{itemize}

\section*{Exercises 15.7}
\begin{itemize}
    \item [1.)] \begin{itemize}
        \item [a.)] \[x=r\cos\theta=4\cos(\pi/3)=2,\,y=r\sin\theta=4\sin(\pi/3)=2\sqrt3,\,z=-2\]
        \[\therefore\ (4,\pi/3,-2)\to(2,2\sqrt3,-2)\]

        \item [b.)] \[x=2\cos(-\pi/2)=0,\,y=2\sin(-\pi/2)=-2,z=1\]
        \[\therefore\ (2,-\pi/2,1)\to(0,-2,1)\]
    \end{itemize}

    \item [3.)] \begin{itemize}
        \item [a.)] \[x=-1,\,y=1,\,r=\sqrt{x^2+y^2}=\sqrt{2},\,\theta=\tan^{-1}(-1)=3\pi/4\]
        \[\therefore\ (-1,1,1)\to(\sqrt2,3\pi/4,1)\]

        \item [b.)] \[x=-2,\,y=2\sqrt3,\,r=\sqrt{4+12}=4,\,\theta=\tan^{-1}(-\sqrt3)=2\pi/3\]
        \[\therefore\ (-2,2\sqrt3,3)\to(4,2\pi/3,3)\]
    \end{itemize}

    \item [9.)] \begin{itemize}
        \item [a.)] \[x^2-x+y^2+z^2=r^2-x-z^2=r^2-r\cos\theta-z^2=1\implies z^2=1-r\cos\theta+r^2\]

        \item [b.)] \[z=x^2-y^2=r^2\cos^2\theta-r^2\sin^2\theta=r^2\cos(2\theta)\]
    \end{itemize}

    \item [17.)] Since $x^2+y^2=16$ represents a circle with radius 4, $0\leq r\leq4$, and $0\leq\theta\leq2\pi$. In addition, $-5\leq z\leq4$. Evaluating the integral:
    \[I=\int^4_{-5}\int^{2\pi}_0\int^4_0r^2\,dr\,d\theta\,dz=\int^4_{-5}\int^{2\pi}_0\bracks{\frac{1}{3}r^3}^4_0\,d\theta\,dz=\int^4_{-5}\int^{2\pi}_0\frac{64}{3}\,d\theta\,dz\]
    \[=\int^4_{-5}\bracks{\frac{64}{3}\theta}^{2\pi}_0\,dz=\int^4_{-5}\frac{128\pi}{3}\,dz=\frac{128\pi}{3}(4+5)=3(128\pi)=384\pi\]

    \item [23.)] 

    \item [24.)]

    \item [29.)] \[I=\int^{2\pi}_0\int^2_0\int^2_rzr^2\cos\theta\,dz\,dr\,d\theta=\int^{2\pi}_0\int^2_0\bracks{\frac{1}{2}z^2r^2\cos\theta}^2_r\,dr\,d\theta\]
    \[=\int^{2\pi}_0\bracks{\frac{2}{3}r^3\cos\theta-\frac{1}{10}r^5\cos\theta}^2_0\,d\theta=\int^{2\pi}_0\frac{16}{3}\cos\theta-\frac{16}{5}\cos\theta\,d\theta=0-0=0\]

\end{itemize}
\end{document}
