\documentclass[12pt]{article}
\pagenumbering{gobble}

\usepackage{amsfonts}
\usepackage{amsmath}
\usepackage{amssymb}
\usepackage{array}
\usepackage{fancyhdr}
\usepackage{mathtools}
\usepackage{textcomp}
\usepackage[margin=1in,headheight=1in]{geometry}

\newcommand{\contradiction}{
    \ensuremath{{\Rightarrow\mspace{-2mu}\Leftarrow}}
}

\newcommand{\angleb}[1]{\left\langle#1\right\rangle}
\newcommand{\vertb}[1]{\left\vert#1\right\vert}
\newcommand{\bracks}[1]{\left[#1\right]}
\newcommand{\parns}[1]{\left(#1\right)}

\newcommand{\lp}{\mathcal{L}}

\newcommand{\derv}[2]{\dfrac{d#1}{d#2}}
\newcommand{\pderv}[2]{\dfrac{\partial#1}{\partial#2}}

\begin{document}
\pagestyle{fancy}
\fancyhead{}
\fancyhead[L]{Alexander Agruso}
\fancyhead[R]{MATH 3323 Homework 17}

\normalsize
\begin{itemize}
    \item [1.)] \[\lp\bracks{t\cos(3t)}=-\frac{d}{ds}\,\frac{s}{s^2+9}=-\frac{s^2+9-2s^2}{(s^2+9)^2}=-\frac{9-s^2}{(s^2+9)^2}\]

    \item [2.)] \[\lp\bracks{t\sin(5t)}=-\frac{d}{ds}\,\frac{5}{s^2+25}=-\frac{-10s}{(s^2+25)^2}=\frac{10s}{(s^2+25)^2}\]
    
    \item [3.)] \[\lp\bracks{t^2\sin t}=(-1)^2\frac{d^2}{ds^2}\,\frac{1}{s^2+1}=\frac{d}{ds}\frac{-2s}{(s^2+1)^2}\]
    \[=\frac{-2(s^2+1)^2+2s(2s)(s^2+1)+2s(s^2+1)(2s)}{(s^2+1)^4}=\frac{-2(s^2+1)^2+4s+4s}{(s^2+1)^3}\]
    \[=-\frac{2(s^2+1)^2+8s}{(s^2+1)^3}\]
    
    \item [4.)] \[\lp\bracks{te^{4t}\cos(3t)}=-\frac{d}{ds}F(s-4)=-\frac{d}{ds}\,\frac{s-4}{(s-4)^2+9}=-\frac{(s-4)^2-(s-4)(2s-8)}{(s^2-8s+25)^2}\]
    \[=-\frac{s^2-8s+25-2s^2+8s+8s-32}{(s^2-8s+25)^2}=\frac{s^2-8s+7}{(s^2-8s+25)^2}\]
    
    \item [5.)] \[\lp\bracks{te^{-3t}\sin t}=-\dfrac{d}{ds}F(s+3)=-\frac{d}{ds}\,\frac{1}{(s+3)^2+1}=-\frac{2s+6}{(s^2+6s+10)^2}\]
    
    \item [6.)] \[\lp\bracks{(t^2+2)^2e^{-2t}}=\lp\bracks{(t^4+4t^2+4)e^{-2t}}=\lp\bracks{t^4e^{-2t}+4t^2e^{-2t}+4e^{-2t}}\]
    \[\frac{d^4}{ds^4}\frac{1}{s+2}+4\frac{d^2}{ds^2}\frac{1}{s+2}+\frac{4}{s+2}=\frac{24}{(s+2)^5}+\frac{8}{(s+2)^3}+\frac{4}{s+2}\]
    
    \item [7.)] \[\lp\bracks{t^9e^{-3t}}=-\frac{d^9}{ds^9}\frac{1}{s+3}=\frac{9!}{(s+3)^{10}}\]
    
    \item [8.)] \[\lp\bracks{t\sinh(2t)\sin(3t)}=-\frac{1}{2}\frac{d}{ds}\lp\bracks{(e^{3t}+e^{-3t})\sin(3t)}\]
    \[=-\frac{1}{2}\frac{d}{ds}\parns{\frac{3}{(s-3)^2+9}+\frac{3}{(s+3)^2+9}}=\frac{1}{2}\parns{\frac{2s-6}{\parns{(s-3)^2+9}^2}+\frac{2s+6}{\parns{(s+3)^2+9}^2}}\]
    
    \item [9.)] \[\lp\bracks{(t+2)e^{-2t}\sin t}=\lp\bracks{te^{-2t}\sin t+2e^{-2t}\sin t}\]
    \[=-\dfrac{d}{ds}\frac{1}{(s+2)^2+1}+\frac{2}{(s+2)^2+1}=\frac{2s+4}{\parns{(s+2)^2+1}^2}+\frac{2}{(s+2)^2+1}\]
    
    \item [10.)] \[\lp\bracks{\int^t_0x^2+\cos x\,dx}=\frac{1}{s}\parns{\frac{2}{s^3}+\frac{s}{s^2+1}}=\frac{2}{s^4}+\frac{1}{s^2+1}\]
    
    \item [11.)] \[\lp\bracks{\int^t_0xe^{-3x}\sin x\,dx}=\frac{1}{s}\lp\bracks{te^{-3t}\sin t}=-\frac{2s+6}{s(s^2+6s+10)^2}\]
    
    \item [12.)] \[\lp\bracks{e^t\int^t_0\cos x\,dx}=\frac{1}{s-1}F(s-1)=\frac{s-1}{(s-1)((s-1)^2+1)}=\frac{1}{(s-1)^2+1}\]
    
\end{itemize}
\end{document}
