\documentclass[12pt]{article}
\pagenumbering{gobble}

\usepackage{amsfonts}
\usepackage{amsmath}
\usepackage{amssymb}
\usepackage{array}
\usepackage{fancyhdr}
\usepackage{mathtools}
\usepackage{textcomp}
\usepackage[margin=1in,headheight=1in]{geometry}

\newcommand{\contradiction}{
    \ensuremath{{\Rightarrow\mspace{-2mu}\Leftarrow}}
}

\newcommand{\angleb}[1]{\left\langle#1\right\rangle}
\newcommand{\vertb}[1]{\left\vert#1\right\vert}
\newcommand{\bracks}[1]{\left[#1\right]}
\newcommand{\parns}[1]{\left(#1\right)}

\newcommand{\derv}[2]{\dfrac{d#1}{d#2}}
\newcommand{\pderv}[2]{\dfrac{\partial#1}{\partial#2}}

\begin{document}
\pagestyle{fancy}
\fancyhead{}
\fancyhead[L]{Alexander Agruso}
\fancyhead[R]{MATH 3323 Homework 12}

\normalsize
\section*{Section 3.5}
\begin{itemize}
    \item [1.)] Find the homogeneous solution:
    \[y''-2y'-3y=0\implies r^2-2r-3=(r-3)(r+1)\implies r=3,-1\]
    \[\therefore y_h=c_1e^{3t}+c_2e^{-t}\]
    Now find $Y$:
    \[g(t)=3e^{2t}\implies Y=Ae^{2t}\]
    \[\therefore\ Y'=2Ae^{2t},\ Y''=4Ae^{2t}\]
    Substituting $y$ with $Y$:
    \[Y''-2Y'-3Y=4Ae^{2t}-4Ae^{2t}-3Ae^{2t}=3e^{2t}\implies 4A-4A-3A=3\]
    \[\implies-3A=3\implies A=-1\]
    \[\therefore y_h+Y=c_1e^{3t}+c_2e^{-t}-e^{2t}\]
    Which is the general solution.

    \item [2.)] Find the homogeneous solution:
    \[y''-y'-2y=0\implies r^2-r-2=(r-2)(r+1)\implies r=2,-1\]
    \[\therefore\ y_h=c_1e^{2t}+c_2e^{-t}\]
    Now find $Y$:
    \[g(t)=-2t+4t^2\implies Y=A+Bt+Ct^2\]
    \[\therefore Y'=B+2Ct,\ Y''=2C\]
    Substituting $y$ with $Y$:
    \[Y''-Y'-2Y=2C-B-2Ct-2A-2Bt-2Ct^2=-2Ct^2-2Bt-2Ct-2A-B+2C\]
    \[\therefore\ -2Ct^2=4t^2\implies C=-2\]
    \[\therefore\ -2Bt-2Ct=-2t\implies-2Bt+4t=-2t\implies-2Bt=-6t\implies B=3\]
    \[\therefore\ -2A-B+2C=-2A-3-4=0\implies-2A=7\implies A=-\frac{7}{2}\]
    \[\therefore\ y_h+Y=c_1e^{2t}+c_2e^{-t}-\frac{7}{2}+3t-2t^2\]
    Which is the general solution.

    \item [5.)] Find the homogeneous solution:
    \[y''+2y'=0\implies r^2+2r=r(r+2)\implies r=0,-2\]
    \[\implies y_h=c_1e^0+c_2e^{-2t}=c_1+c_2e^{-2t}\]
    Now find $Y$:
    \[g(t)=3+4\sin(2t)\implies Y=At+B\sin(2t)+C\cos(2t)\]
    \[\therefore\ Y'=A+2B\cos(2t)-2C\sin(2t),\ Y''=-4B\sin(2t)-4C\cos(2t)\]
    Substituting $y$ with $Y$:
    \[Y''+2Y'=-4B\sin(2t)-4C\cos(2t)+2A+4B\cos(2t)-4C\sin(2t)\]
    \[\therefore\ 2A=3\implies A=\frac{3}{2}\]
    \[\therefore\ -4B-4C=4\implies -B-C=1\implies C=-B-1\]
    \[\therefore\ 4B-4C=4B-4(-B-1)=4B+4B+4=0\implies8B=-4\implies B=-\frac{1}{2}\]
    \[\therefore\ -4B-4C=2-4C=4\implies C=-\frac{2}{4}=-\frac{1}{2}\]
    \[\therefore y_h+Y=c_1+c_2e^{-2t}+\frac{3}{2}t-\frac{1}{2}\sin(2t)-\frac{1}{2}\cos(2t)\]
    Which is the general solution.
    
    \item [10.)] Find the homogeneous solution:
    \[y''+y'+4y=0\implies r^2+r+4\implies r=\frac{-1\pm\sqrt{1-16}}{2}=\frac{-1\pm\sqrt{15}i}{2}\]
    \[\implies \lambda=-\frac{1}{2},\ \mu=\sqrt{15}\]
    \[\therefore\ y_h=c_1e^{-t/2}\cos\parns{\sqrt{15}t}+c_2e^{-t/2}\sin\parns{\sqrt{15}t}\]
    Now find $Y$:
    \[g(t)=2\sinh t=e^t-e^{-t}\implies Y=Ae^t+Be^{-t}\]
    \[\therefore\ Y'=Ae^t-Be^{-t},\ Y''=Ae^t+Be^{-t}\]
    Substituting $y$ with $Y$:
    \[Y''+Y'+4Y=Ae^t+Be^{-t}+Ae^t-Be^{-t}+4Ae^t+4Be^{-t}=6Ae^t+4Be^{-t}\]
    \[\therefore\ 6A=1\implies A=\frac{1}{6}\]
    \[\therefore\ 4B=-1\implies B=-\frac{1}{4}\]
    \[\therefore\ y_h+Y=c_1e^{-t/2}\cos\parns{\sqrt{15}t}+c_2e^{-t/2}\sin\parns{\sqrt{15}t}+\frac{1}{6}e^t-\frac{1}{4}e^{-t}\]
    Which is the general solution.

    \item [11.)] Find the homogeneous solution:
    \[y''+y'-2y=0\implies r^2+r-2=(r+2)(r-1)\implies r=-2,1\]
    \[\therefore\ y_h=c_1e^t+c_2e^{-2t}\]
    Now find $Y$:
    \[g(t)=2t\implies Y=A+Bt\]
    \[\therefore\ Y'=B,\ Y''=0\]
    Substituting $y$ with $Y$:
    \[Y''+Y'-2Y=0+B-2A-2Bt=2t\]
    \[\therefore\ B-2A=0\implies B=2A\]
    \[\therefore\ -2B=2\implies B=-1\implies A=-\frac{1}{2}\]
    \[\therefore\ y_h+Y=c_1e^t+c_2e^{-2t}-\frac{1}{2}-t\]
    \[\therefore\ (y_h+Y)'=c_1e^t-2c_2e^{-2t}-1\]
    Which is the general solution. We can solve for $c_1$ and $c_2$ given initial conditions $y(0)=0$ and $y'(0)=1$:
    \[0=c_1e^{0}+c_2e^{-2(0)}-\frac{1}{2}-0=c_1+c_2-\frac{1}{2}\implies\frac{1}{2}=c_1+c_2\]
    \[1=c_1e^0-2c_2e^{-2(0)}-1\implies2=c_1-2c_2\implies c_1=2c_2+2\]
    \[\implies\frac{1}{2}=2c_2+2+c_2=3c_2+2\implies-\frac{3}{2}=3c_2\implies c_2=-\frac{1}{2}\]
    \[\implies\frac{1}{2}=c_1-\frac{1}{2}\implies c_1=1\]
    \[\therefore\ y_h+Y=e^t-\frac{1}{2}e^{-2t}-\frac{1}{2}-t\]
    Which is the particular solution.

    \item [16.)] Given $y_h=c_1+c_2e^{-3t}$, and given $g(t)=2t^4+t^2e^{-3t}+\sin(3t)$, we can determine the form of the particular solution to be as follows:
    \[Y=t(A+Bt+Ct^2+Dt^3+Et^4)+t(F+Gt+Ht^2)e^{-3t}+I\sin(3t)+J\cos(3t)\]

    \item [19.)] Given $y_h=c_1+c_2e^{-4t}$, and given $g(t)=t^2\sin(2t)+(6t+7)\cos(2t)$, we can determine the form of the particular solution to be as follows:
    \[Y=t(A+Bt+Ct^2)(D\sin(2t)+E\cos(2t))+t(F+Gt+Ht^2)(I\sin(2t)+J\cos(2t))\]
    \[=t(A+Bt+Ct^2)\sin(2t)+t(D+Et+Ft^2)\cos(2t)\]
\end{itemize}
\end{document}
