\documentclass[12pt]{article}
\pagenumbering{gobble}
\linespread{1.15}

\usepackage{amsfonts}
\usepackage{amsmath}
\usepackage{amssymb}
\usepackage{array}
\usepackage{fancyhdr}
\usepackage{textcomp}
\usepackage[margin=1in,headheight=1in]{geometry}

\newcommand{\contradiction}{
    \ensuremath{{\Rightarrow\mspace{-2mu}\Leftarrow}}
}

\newcommand{\angleb}[1]{\left\langle#1\right\rangle}
\newcommand{\vertb}[1]{\left\vert#1\right\vert}
\newcommand{\bracks}[1]{\left[#1\right]}

\newcommand{\derv}[2]{\dfrac{d#1}{d#2}}

\begin{document}
\pagestyle{fancy}
\fancyhead{}
\fancyhead[L]{Alexander Agruso}
\fancyhead[R]{MATH 3323 Extra Credit 1}

\normalsize
\begin{itemize}
    \item [1.)] Manipulate to a function of $\dfrac{y}{x}$:
    \[\frac{dy}{dx}=\frac{x^2+xy+y^2}{x^2}=1+\frac{y}{x}+\frac{y^2}{x^2}\]
    Substitute $y=ux$:
    \[u+x\frac{du}{dx}=1+u+u^2\implies x\frac{du}{dx}=1+u^2\]
    Separate:
    \[x\frac{du}{dx}=1+u^2\implies\frac{du}{1+u^2}=\frac{dx}{x}\]
    Solve for $u$:
    \[\int\frac{du}{1+u^2}=\arctan{u}=\int\frac{dx}{x}=\ln\vert x\vert+C\implies u=\tan(\ln\vert x\vert+C)\]
    Replace $u=\dfrac{y}{x}$ and solve for $y$:
    \[\frac{y}{x}=\tan(\ln\vert x\vert+C)\implies y=x\tan(\ln\vert x\vert+C)\]
    Which is the explicit solution.

    \item [2.)] Manipulate to a function of $\dfrac{y}{x}$:
    \[(x^2+3xy+y^2)dx-x^2dy=0\implies\frac{dy}{dx}=\frac{x^2+3xy+y^2}{x^2}=1+\frac{3y}{x}+\frac{y^2}{x^2}\]
    Substitute $y=ux$:
    \[u+x\frac{du}{dx}=1+3u+u^2\implies x\frac{du}{dx}=1+2u+u^2=(1+u)^2\]
    Separate:
    \[x\frac{du}{dx}=(1+u)^2\implies\frac{du}{(1+u)^2}=\frac{dx}{x}\]
    Solve for $u$:
    \[\int\frac{du}{(1+u)^2}=-\frac{1}{1+u}=\int\frac{dx}{x}=\ln\vert x\vert+C\implies-1-u=\frac{1}{\ln\vert x\vert+C}\]
    \[\implies u=-\frac{1}{\ln\vert x\vert+C}-1\]
    Replace $u=\dfrac{y}{x}$ and solve for $y$:
    \[\frac{y}{x}=-\frac{1}{\ln\vert x\vert+C}-1\implies y=-\frac{x}{\ln\vert x\vert+C}-x\]
    Which is the explicit solution.

    \pagebreak
    \item [3.)] Manipulate to a function of $\dfrac{y}{x}$:
    \[x\frac{dy}{dx}=y+x\tan\left(\frac{y}{x}\right)\implies\frac{dy}{dx}=\frac{y}{x}+\tan\left(\frac{y}{x}\right)\]
    Substitute $y=ux$:
    \[u+x\frac{du}{dx}=u+\tan(u)\implies x\frac{du}{dx}=\tan(u)\]
    Separate:
    \[x\frac{du}{dx}=\tan(u)\implies\cot(u)du=\frac{dx}{x}\]
    Solve for $u$:
    \[\int\cot(u)du=\ln\vert\sin(u)\vert=\int\frac{dx}{x}=\ln\vert x\vert+C\implies u=\arcsin\left(xe^C\right)\]
    Replace $u=\dfrac{y}{x}$ and solve for $y$:
    \[\frac{y}{x}=\arcsin\left(xe^C\right)\implies y=x\arcsin\left(xe^C\right)\]
    Which is the explicit solution.

\end{itemize}

\end{document}
